shared SN term construction
git-svn-id: svn+ssh://scm.gforge.inria.fr/svn/coqcert/trunk/cic-model@135 7b0040dd-6dd6-45fd-888d-7922243e4794

GenModelSN.v
@@ -2,6 +2,7 @@ Set Implicit Arguments.
 Require Import List Compare_dec.
 Require Import Sat.
 Require Import Models.
+Require ObjectSN.
 
 Module Lc := Lambda.
 
@@ -32,401 +33,10 @@ Module MakeModel(M : CC_Model) (SN : SN_addon M).
 Import M.
 Import SN.
 
-(* Valuations *)
-Module Xeq.
-  Definition t := X.
-  Definition eq := eqX.
-  Definition eq_equiv : Equivalence eq := eqX_equiv.
-  Existing Instance eq_equiv.
-End Xeq.
-Require Import VarMap.
-Module V := VarMap.Make(Xeq).
-
-Notation val := V.map.
-Notation eq_val := V.eq_map.
-
-Definition vnil : val := V.nil props.
-
-Import V.
-Existing Instance cons_morph.
-Existing Instance cons_morph'.
-Existing Instance shift_morph.
-Existing Instance lams_morph.
-
-(* Term valuations *)
-Module I := Lambda.I.
-
-(* Terms *)
-
-Record inftrm := {
-  iint : val -> X;
-  iint_morph : Proper (eq_val ==> eqX) iint;
-  itm : Lc.intt -> Lc.term;
-  itm_morph : Proper (Lc.eq_intt ==> eq) itm;
-  itm_lift : Lc.liftable itm;
-  itm_subst : Lc.substitutive itm
-}.
-Existing Instance iint_morph.
-Existing Instance itm_morph.
-
-Definition trm := option inftrm.
-
-Definition eq_trm (x y:trm) :=
-  match x, y with
-  | Some f, Some g =>
-     (eq_val ==> eqX)%signature (iint f) (iint g) /\
-     (Lc.eq_intt ==> eq)%signature (itm f) (itm g)
-  | None, None => True
-  | _, _ => False
-  end.
-
-Instance eq_trm_refl : Reflexive eq_trm.
-red; intros.
-destruct x as [(f,mf,g,mg,sg)|]; simpl; auto.
-Qed.
-
-Instance eq_trm_sym : Symmetric eq_trm.
-red; intros.
-destruct x as [(fx,mfx,gx,mgx,sgx)|];
-destruct y as [(fy,mfy,gy,mgy,sgy)|]; simpl in *; auto.
-destruct H; split; symmetry; trivial.
-Qed.
-
-Instance eq_trm_trans : Transitive eq_trm.
-red; intros.
-destruct x as [(fx,mfx,gx,mgx,sgx)|];
-destruct y as [(fy,mfy,gy,mgy,sgy)|];
-destruct z as [(fz,mfz,gz,mgz,sgz)|];
- try contradiction; simpl in *; auto.
-destruct H; destruct H0; split.
- transitivity fy; trivial.
- transitivity gy; trivial.
-Qed.
-
-Lemma eq_kind : forall (M:trm), M = None <-> eq_trm M None.
-destruct M; simpl; split; contradiction||discriminate||trivial.
-Qed.
-
-Definition tm (j:Lc.intt) (M:trm) :=
-  match M with
-  | Some f => itm f j
-  | None => Lc.K (* kind is interpreted by any SN term *)
-  end.
-
-Definition int (i:val) (M:trm) :=
-  match M with
-  | Some f => iint f i
-  | None => props
-  end.
-
-Lemma eq_trm_intro : forall T T',
-  (forall i, int i T == int i T') ->
-  (forall j, tm j T = tm j T') ->
-  match T, T' with Some _,Some _=>True|None,None=>True|_,_=>False end ->
-  eq_trm T T'.
-destruct T as [T|]; destruct T' as [T'|]; simpl; intros; trivial.
-split; red; intros.
- rewrite H2; auto.
- rewrite H2; auto.
-Qed.
-
-Instance tm_morph : Proper (Lc.eq_intt ==> eq_trm ==> eq) tm.
-unfold tm; do 3 red; intros.
-destruct x0; destruct y0; simpl in *; (contradiction||reflexivity||auto).
-destruct H0; simpl in *.
-apply H1; trivial.
-Qed.
-
-Lemma tm_substitutive : forall u t j k,
-  tm (fun n => Lc.subst_rec u (j n) k) t =
-  Lc.subst_rec u (tm j t) k.
-destruct t; simpl; intros; trivial.
-apply itm_subst.
-Qed.
-
-Lemma tm_liftable : forall j t k,
-  tm (fun n => Lc.lift_rec 1 (j n) k) t = Lc.lift_rec 1 (tm j t) k.
-destruct t; simpl; intros; trivial.
-apply itm_lift.
-Qed.
-
-Lemma tm_subst_cons : forall x j t,
-  tm (I.cons x j) t = Lc.subst x (tm (Lc.ilift j) t).
-unfold Lc.subst; intros.
-rewrite <- tm_substitutive.
-apply tm_morph; [red; intros|reflexivity].
-red.
-destruct a; simpl.
- rewrite Lc.lift0; trivial.
- rewrite Lc.simpl_subst; trivial; rewrite Lc.lift0; trivial.
-Qed.
-
-Instance int_morph : Proper (eq_val ==> eq_trm ==> eqX) int.
-unfold int; do 3 red; intros.
-destruct x0; destruct y0; simpl in *; (contradiction||reflexivity||auto).
-destruct H0; simpl in *.
-apply H0; trivial.
-Qed.
-
-Definition kind : trm := None.
-
-Definition prop : trm.
-left; exists (fun _ => props) (fun _=> Lc.K).
- do 2 red; reflexivity.
- do 2 red; reflexivity.
- red; reflexivity.
- red; reflexivity.
-Defined.
-
-Definition Ref (n:nat) : trm.
-left; exists (fun i => i n) (fun j => j n).
- do 2 red; simpl; auto.
- do 2 red; simpl; auto.
- red; reflexivity.
- red; reflexivity.
-Defined.
-
-Definition App (u v:trm) : trm.
-left; exists (fun i => app (int i u) (int i v))
-             (fun j => Lc.App (tm j u) (tm j v)). 
- do 2 red; simpl; intros.
- rewrite H; reflexivity.
-
- do 2 red; simpl; intros.
- rewrite H; reflexivity.
-
- red; simpl; intros.
- do 2 rewrite <- tm_liftable; trivial.
-
- red; simpl; intros.
- do 2 rewrite <- tm_substitutive; trivial.
-Defined.
-
-Definition Abs (A M:trm) : trm.
-left; exists (fun i => lam (int i A) (fun x => int (V.cons x i) M))
-             (fun j => Lc.App2 Lc.K (Lc.Abs (tm (Lc.ilift j) M)) (tm j A)).
- do 2 red; simpl; intros.
- apply lam_ext.
-  rewrite H; reflexivity.
-
-  red; intros.
-  rewrite H; rewrite H1; reflexivity.
-
- do 2 red; intros.
- rewrite H; trivial.
-
- red; simpl; intros.
- rewrite Lc.ilift_binder_lift; trivial.
- do 2 rewrite <- tm_liftable; trivial.
-
- red; simpl; intros.
- rewrite Lc.ilift_binder; trivial.
- do 2 rewrite <- tm_substitutive; trivial.
-Defined.
-
-Definition Prod (A B:trm) : trm.
-left;
-  exists (fun i => prod (int i A) (fun x => int (V.cons x i) B))
-         (fun j => Lc.App2 Lc.K (tm j A) (Lc.Abs (tm (Lc.ilift j) B))).
-do 2 red; simpl; intros.
- apply prod_ext.
-  rewrite H; reflexivity.
-
-  red; intros.
-  rewrite H; rewrite H1; reflexivity.
-
- do 2 red; intros.
- rewrite H; trivial.
-
- red; simpl; intros.
- do 2 rewrite <- tm_liftable; trivial.
- rewrite Lc.ilift_binder_lift; trivial.
-
- red; simpl; intros.
- do 2 rewrite <- tm_substitutive; trivial.
- rewrite Lc.ilift_binder; trivial.
-Defined.
-
-Definition lift_rec (n m:nat) (t:trm) : trm.
-destruct t as [t|]; [left|exact kind].
-exists (fun i => iint t (V.lams m (V.shift n) i))
-       (fun j => itm t (I.lams m (I.shift n) j)).
- do 2 red; intros.
- rewrite H; reflexivity.
-
- do 2 red; intros.
- rewrite H; reflexivity.
-
- red; intros.
- rewrite <- itm_lift.
- apply itm_morph; do 2 red; intros.
- unfold I.lams.
- destruct (le_gt_dec m a); trivial.
-
- red; intros.
- rewrite <- itm_subst.
- apply itm_morph; do 2 red; intros.
- unfold I.lams.
- destruct (le_gt_dec m a); trivial.
-Defined.
-
-Lemma int_lift_rec_eq : forall n k T i,
-  int i (lift_rec n k T) == int (V.lams k (V.shift n) i) T.
-intros; destruct T as [T|]; simpl; reflexivity.
-Qed.
-
-Definition lift n := lift_rec n 0.
-
-Instance lift_morph : forall k, Proper (eq_trm ==> eq_trm) (lift k).
-do 2 red; simpl; intros.
-destruct x as [x|]; destruct y as [y|];
-  simpl in *; (contradiction||trivial).
-destruct H; split.
- red; intros.
- apply H; rewrite H1; reflexivity.
-
- red; intros.
- apply H0; rewrite H1; reflexivity.
-Qed.
-
-Lemma int_lift_eq : forall i T,
-  int i (lift 1 T) == int (V.shift 1 i) T.
-unfold int; intros;
-  destruct T as [T|]; simpl; auto. (* BUG: intros needed before destruct *)
-2:reflexivity.
-rewrite V.lams0.
-reflexivity.
-Qed.
-
-Lemma int_cons_lift_eq : forall i T x,
-  int (V.cons x i) (lift 1 T) == int i T.
-intros.
-rewrite int_lift_eq.
-rewrite V.shift_cons; reflexivity.
-Qed.
-
-Lemma tm_lift_rec_eq : forall n k T j,
-  tm j (lift_rec n k T) = tm (I.lams k (I.shift n) j) T.
-intros; destruct T; simpl; reflexivity.
-Qed.
-
-Lemma split_lift : forall n T,
-  eq_trm (lift (S n) T) (lift 1 (lift n T)).
-destruct T as [T|]; simpl; auto.
-split; red; intros.
- do 2 rewrite V.lams0.
- change (V.shift n (fun k => V.lams 0 (V.shift 1) y k)) with
-   (V.shift n (V.lams 0 (V.shift 1) y)).
- rewrite V.lams0.
- rewrite V.shift_split.
- change (eq_val (fun k => x k) (fun k => y k)) in H.
- rewrite H; reflexivity.
-
- do 2 rewrite I.lams0.
- change (I.shift n (fun k => I.lams 0 (I.shift 1) y k)) with
-   (I.shift n (I.lams 0 (I.shift 1) y)).
- rewrite I.lams0.
- rewrite I.shift_split.
- change (Lc.eq_intt (fun k => x k) (fun k => y k)) in H.
- rewrite H; reflexivity.
-Qed.
-
-Definition subst_rec (arg:trm) (m:nat) (t:trm) : trm.
-destruct t as [body|]; [left|right].
-exists (fun i => iint body (V.lams m (V.cons (int (V.shift m i) arg)) i))
-       (fun j => itm body (I.lams m (I.cons (tm (I.shift m j) arg)) j)).
- do 2 red; intros.
- rewrite H; reflexivity.
-
- do 2 red; intros.
- rewrite H; reflexivity.
-
- red; intros.
- rewrite <- itm_lift.
- apply itm_morph; do 2 red; intros.
- unfold I.lams.
- destruct (le_gt_dec m a); trivial.
- destruct (a-m); simpl; auto.
- rewrite <- tm_liftable.
- reflexivity.
-
- red; intros.
- rewrite <- itm_subst.
- apply itm_morph; do 2 red; intros.
- unfold I.lams.
- destruct (le_gt_dec m a); trivial.
- destruct (a-m); simpl; auto.
- rewrite <- tm_substitutive.
- reflexivity.
-Defined.
-
-Lemma int_subst_rec_eq : forall arg k T i,
-  int i (subst_rec arg k T) == int (V.lams k (V.cons (int (V.shift k i) arg)) i) T.
-intros; destruct T as [T|]; simpl; reflexivity.
-Qed.
-
-Definition subst arg := subst_rec arg 0.
-
-Lemma int_subst_eq : forall N M i,
- int (V.cons (int i N) i) M == int i (subst N M).
-destruct M as [M|]; simpl; intros.
-2:reflexivity.
-rewrite V.lams0.
-rewrite V.shift0.
-reflexivity.
-Qed.
-
-Lemma tm_subst_rec_eq : forall arg k T j,
-  tm j (subst_rec arg k T) = tm (I.lams k (I.cons (tm (I.shift k j) arg)) j) T.
-intros; destruct T; simpl; reflexivity.
-Qed.
-
-Lemma tm_subst_eq : forall u v j,
-  tm j (subst u v) = Lc.subst (tm j u) (tm (Lc.ilift j) v).
-intros.
-unfold Lc.subst; rewrite <- tm_substitutive.
-destruct v as [v|]; simpl; trivial.
-rewrite I.lams0.
-rewrite I.shift0.
-apply itm_morph.
-apply I.cons_ext; simpl.
- rewrite Lc.lift0; trivial.
-
- do 2 red; unfold I.shift; simpl; intros.
- rewrite Lc.simpl_subst; trivial; rewrite Lc.lift0; trivial.
-Qed.
-
-Instance App_morph : Proper (eq_trm ==> eq_trm ==> eq_trm) App.
-unfold App; do 3 red; simpl; split; intros.
- red; intros.
- rewrite H; rewrite H0; rewrite H1; reflexivity.
-
- red; intros.
- rewrite H; rewrite H0; rewrite H1; reflexivity.
-Qed.
-
-Instance Abs_morph : Proper (eq_trm ==> eq_trm ==> eq_trm) Abs.
-unfold Abs; do 4 red; simpl; split; red; intros.
- apply lam_ext.
-  apply int_morph; auto.
-
-  red; intros.
-  rewrite H0; rewrite H1; rewrite H3; reflexivity.
-
- rewrite H0; rewrite H1; rewrite H; reflexivity.
-Qed.
-
-
-Instance Prod_morph : Proper (eq_trm ==> eq_trm ==> eq_trm) Prod.
-unfold Prod; do 4 red; simpl; split; red; intros.
- apply prod_ext.
-  rewrite H; rewrite H1; reflexivity.
-
-  red; intros.
-  rewrite H0; rewrite H1; rewrite H3; reflexivity.
-
- rewrite H0; rewrite H1; rewrite H; reflexivity.
-Qed.
+(* We use the generic model construction upon the
+   abstract model
+ *)
+Include ObjectSN.MakeObject(M).
 
 
 (* Dealing with top sorts *)
@@ -449,12 +59,6 @@ apply lam_ext; intros.
  apply IHx0.
  rewrite H2; rewrite H; reflexivity.
 Qed.
-
-Fixpoint prod_list (e:list trm) (U:trm) :=
-  match e with
-  | List.nil => U
-  | T::f => Prod T (prod_list f U)
-  end.
 
 Lemma wit_prod : forall x U,
   (forall i, x \in int i U) ->
@@ -512,57 +116,43 @@ rewrite eq_U.
 apply wit_prod; trivial.
 Qed.
 
-Lemma discr_ref_prod : forall n A B,
-  ~ eq_trm (Ref n) (Prod A B).
-red; intros.
-simpl in H.
-destruct H as (_,H).
-red in H.
-specialize H with Lc.Ref Lc.Ref.
-discriminate H.
-reflexivity.
-Qed.
-
-Lemma lift1var : forall n, eq_trm (lift 1 (Ref n)) (Ref (S n)).
-simpl; split; red; intros.
- revert n.
- change (eq_val (V.lams 0 (V.shift 1) x) (V.shift 1 y)).
- rewrite V.lams0; rewrite <- H.
- reflexivity.
-
- revert n.
- change (Lc.eq_intt (I.lams 0 (I.shift 1) x) (I.shift 1 y)).
- rewrite I.lams0; rewrite <- H.
- reflexivity.
-Qed.
-
-Lemma non_empty_var_lift : forall n,
-  non_empty (Ref n) -> non_empty (Ref (S n)).
-intros n (e,(U,eq_U,(x,in_U))).
-destruct e; simpl prod_list in eq_U.
- exists List.nil; exists (lift 1 U).
-  simpl prod_list.
-  rewrite <- lift1var.
-  apply lift_morph; trivial.
+Lemma non_empty_lift M k :
+  non_empty M <-> non_empty (lift_rec 1 k M).
+unfold non_empty; split; intros.
+ destruct H as (e,(U,?,(x,?))).
+ destruct lift_prod_list_ex with 1 k e U as (e',?).
+ exists e'.
+ exists (lift_rec 1 (length e+k) U).
+  rewrite H; trivial.
 
   exists x; intros.
-  setoid_replace i with (V.cons (i 0) (V.shift 1 i)).
-   rewrite int_lift_eq; trivial.
+  rewrite int_lift_rec_eq.
+  apply H0.
 
-   red; intros.
-   destruct a; reflexivity.
+ destruct H as (e,(U,?,(x,?))).
+ destruct subst_prod_list_ex with (Ref 0) k e U as (e',?).
+ exists e'.
+ exists (subst_rec (Ref 0) (length e+k) U).
+  rewrite <- H1.
+  rewrite <- H.
+  apply simpl_subst_lift_rec.
 
- elim (discr_ref_prod eq_U).
+  exists x; intros.
+  rewrite int_subst_rec_eq.
+  apply H0.
 Qed.
 
 
+(* Semantic typing relation.
+   Handles the case of kind: a type that contains all "non-empty" types
+   and that is included in no type.
+ *)
 Definition in_int (i:val) (j:Lc.intt) (M T:trm) :=
   M <> None /\
   match T with
-  | None => non_empty M
-  | _ => int i M \in int i T
-  end /\
-  inSAT (tm j M) (Red (int i T)).
+  | None => non_empty M /\ Lc.sn (tm j M)
+  | _ => int i M \in int i T /\ inSAT (tm j M) (Red (int i T))
+  end.
 
 Instance in_int_morph : Proper
   (eq_val ==> pointwise_relation nat (@eq Lc.term) ==> eq_trm ==> eq_trm ==> iff)
@@ -574,7 +164,7 @@ destruct x2; destruct y2; try contradiction.
  rewrite H; rewrite H0; rewrite H1; rewrite H2.
  reflexivity.
 
- rewrite H; rewrite H0; rewrite H1.
+ rewrite H0; rewrite H1.
  reflexivity.
 Qed.
 
@@ -583,9 +173,8 @@ Lemma in_int_not_kind : forall i j M T,
   T <> kind ->
   int i M \in int i T /\
   inSAT (tm j M) (Red (int i T)).
-destruct 1 as (_,(mem,sat)); intros.
-destruct T; auto.
-elim H; trivial.
+destruct T; intros in_T not_tops;[|elim not_tops; reflexivity].
+destruct in_T as (mem,sat); trivial.
 Qed.
 
 Lemma in_int_intro : forall i j M T,
@@ -607,39 +196,30 @@ Lemma in_int_var0 : forall i j x t T,
   in_int (V.cons x i) (I.cons t j) (Ref 0) (lift 1 T).
 intros.
 red; simpl.
-split; try discriminate.
-split.
- revert H1; pattern T at 1 2.
- case T; simpl; intros.
-  rewrite int_cons_lift_eq; trivial.
-
-  elim H1; trivial.
-
- rewrite int_cons_lift_eq; trivial.
+revert H1; pattern T at 1 2.
+case T; [|destruct 1;reflexivity].
+simpl; intros _ _.
+split; [discriminate|].
+rewrite int_cons_lift_eq; auto.
 Qed.
 
 Lemma in_int_varS : forall i j x t n T,
   in_int i j (Ref n) (lift (S n) T) ->
   in_int (V.cons x i) (I.cons t j) (Ref (S n)) (lift (S (S n)) T).
-intros.
-destruct H as (_,(mem,subs)); simpl in *.
-red; simpl.
-split; try discriminate.
-split.
- revert mem; pattern T at 1 3.
- case T; [intros T0|]; simpl; intros; trivial.
-  rewrite split_lift.
-  rewrite int_cons_lift_eq; trivial.
-
-  apply non_empty_var_lift; trivial.
-
+destruct 1 as (_,in_T); split; [discriminate|].
+revert in_T; pattern T at 1 4; case T; simpl.
+ intros _ in_T.
  rewrite split_lift.
  rewrite int_cons_lift_eq; trivial.
+
+ destruct 1; split; trivial.
+ rewrite non_empty_lift with (k:=0) in H.
+ rewrite eq_trm_lift_ref_fv in H; auto with arith.
 Qed.
 
 Lemma in_int_sn : forall i j M T,
   in_int i j M T -> Lc.sn (tm j M).
-destruct 1 as (_,(_,sat)).
+intros i j M [f|] (_,(_,sat)); trivial.
 apply sat_sn in sat; trivial.
 Qed.
 
@@ -685,6 +265,7 @@ apply varSAT.
 Qed.
 
 (* Judgements *)
+
 Definition wf (e:env) :=
   exists i, exists j, val_ok e i j.
 Definition typ (e:env) (M T:trm) :=
@@ -703,6 +284,30 @@ unfold eq_typ; split; simpl; intros.
  rewrite <- H; rewrite <- H0; eauto.
  rewrite H; rewrite H0; eauto.
 Qed.
+
+(* Strong normalization *)
+
+(* This lemma shows that the abstract model construction entails
+   strong normalization.
+   At this level, we do have the actual syntax. However, red_term
+   is a relation on the denotations that admits the same introduction
+   rules as the syntactic reduction.
+   When the syntax is introduced, it will only remain to check that
+   the syntactic reduction implies the semantic one, which will be
+   straightforward.
+ *)
+Lemma model_strong_normalization e M T :
+  wf e ->
+  typ e M T ->
+  Acc (transp _ red_term) M.
+intros (i,(j,is_val)) ty.
+apply ty in is_val.
+apply in_int_sn in is_val.
+apply simul with (1:=is_val) (2:=eq_refl).
+Qed.
+
+
+(* Well-formed types: terms typed by a sort *)
 
 Definition typs e T :=
   typ e T kind \/ typ e T prop.
@@ -729,17 +334,7 @@ destruct H.
 Qed.
 
 
-(* Strong normalization *)
-
-Lemma typ_sn : forall e M T,
-  wf e -> typ e M T -> exists j, Lc.sn (tm j M).
-intros e M T (i,(j,is_val)) ty.
-exists j.
-apply ty in is_val.
-apply in_int_sn in is_val; trivial.
-Qed.
-
-(* Context formation *)
+(* Context formation rules *)
 
 Lemma wf_nil : wf List.nil.
 red.
@@ -842,6 +437,7 @@ apply H with (j:=I.cons daimon j).
 apply vcons_add_var0; auto.
 Qed.
 
+(* Typing rules *)
 
 Lemma typ_prop : forall e, typ e prop kind.
 red; simpl; intros.
@@ -849,8 +445,6 @@ split; try discriminate.
 split; simpl; auto.
  apply prop_non_empty.
 
- rewrite Red_sort.
- apply snSAT_intro.
  apply Lc.sn_K.
 Qed.
 
@@ -859,7 +453,6 @@ Lemma typ_var : forall e n T,
 red; simpl; intros.
 apply H0 in H; trivial.
 Qed.
-
 
 Lemma typ_app : forall e u v V Ur,
   typ e v V ->
@@ -891,7 +484,6 @@ apply prod_elim with (x:=int i v) in H1; trivial.
  rewrite H4; reflexivity.
 Qed.
 
-
 Lemma typ_abs : forall e T M U,
   typs e T ->
   typ (T :: e) M U ->
@@ -919,8 +511,8 @@ apply in_int_intro; simpl; try discriminate.
  destruct (typs_non_empty ty_T is_val) as (wit,in_T).
  apply KSAT_intro.
   destruct ty_T as [ty_T|ty_T]; apply ty_T in is_val;
-    destruct is_val as (_,(_,satT)); simpl in satT;
-    rewrite Red_sort in satT; trivial.
+    destruct is_val as (_,(_,satT)); simpl in satT; trivial.
+  rewrite Red_sort in satT; trivial.
 
   apply prodSAT_intro; intros.
   apply interSAT_intro; intros.
@@ -963,36 +555,41 @@ destruct (typs_non_empty ty_T is_val) as (witT,in_T).
 specialize vcons_add_var0 with (1:=is_val) (2:=in_T) (3:=T_not_tops);
   intros in_U.
 apply ty_U in in_U.
-split;[discriminate|split;simpl].
- destruct is_srt; subst s2; simpl in *.
-  apply prod_non_empty.
-  destruct in_U as (_,(mem,_)); trivial.
+assert (Lc.sn (tm j T)).
+ destruct ty_T as [ty_T|ty_T]; apply ty_T in is_val;
+   destruct is_val as (_,(_,satT)); trivial.
+ apply sat_sn in satT; trivial.
+split;[discriminate|destruct is_srt; subst s2; split;simpl].
+ (* s2=kind *)
+ (* non_empty: *)
+ apply prod_non_empty.
+ destruct in_U as (_,(mem,_)); trivial.
 
-  apply impredicative_prod; intros.   
-   red; intros.
-   rewrite H1; reflexivity.
-
-   clear in_U.
-   specialize vcons_add_var0 with (1:=is_val) (2:=H0) (3:=T_not_tops);
-     intros in_U.
-   apply ty_U in in_U.
-   apply in_int_not_kind in in_U.
-    destruct in_U; trivial.
-    discriminate.
-
+ (* sn *)
  destruct in_U as (_,(_,satU)).
  rewrite tm_subst_cons in satU.
- apply KSAT_intro.
-  apply Lc.sn_abs.
-  apply sat_sn in satU.
-  apply Lc.sn_subst in satU; trivial.
+ apply Lc.sn_subst in satU.
+ apply KSAT_intro with (A:=snSAT); auto.
 
-  assert (Lc.sn (tm j T)).
-   destruct ty_T as [ty_T|ty_T]; apply ty_T in is_val;
-     destruct is_val as (_,(_,satT));
-     apply sat_sn in satT; trivial.
-  destruct is_srt; subst s2; simpl; rewrite Red_sort;
-    apply snSAT_intro; trivial.
+ (* s2=prop *)
+ (* value *)
+ apply impredicative_prod; intros.   
+  red; intros.
+  rewrite H2; reflexivity.
+
+  clear in_U.
+  specialize vcons_add_var0 with (1:=is_val) (2:=H1) (3:=T_not_tops);
+    intros in_U.
+  apply ty_U in in_U.
+  apply in_int_not_kind in in_U;[|discriminate].
+  destruct in_U; trivial.
+
+ (* sat *)
+ destruct in_U as (_,(_,satU)).
+ rewrite Red_sort in satU|-*; simpl.
+ rewrite tm_subst_cons in satU.
+ apply Lc.sn_subst in satU.
+ apply KSAT_intro with (A:=snSAT); auto.
 Qed.
 
 Lemma typ_conv : forall e M T T',
@@ -1013,288 +610,6 @@ apply in_int_intro; trivial.
 
  rewrite <- H0; trivial.
 Qed.
-
-(* "Untyped" Reduction *)
-Require Import Relations.
-
-Definition red_term M N :=
-  forall j, clos_trans _ Lc.red1 (tm j M) (tm j N).
-
-Instance red_term_morph : Proper (eq_trm ==> eq_trm ==> iff) red_term.
-apply morph_impl_iff2; auto with *.
-do 4 red; intros.
-red; intros.
-rewrite <- H; rewrite <- H0; auto.
-Qed.
-
-Lemma red_term_trans M1 M2 M3 :
-  red_term M1 M2 -> red_term M2 M3 -> red_term M1 M3.
-unfold red_term; intros.
-specialize H with j.
-specialize H0 with j.
-apply t_trans with (tm j M2); trivial.
-Qed.
-
-Lemma red_term_app_l M M' N :
-  red_term M M' ->
-  red_term (App M N) (App M' N).
-unfold red_term; intros.
-specialize H with j.
-apply Lc.redp_app_l; trivial.
-Qed.
-
-
-Lemma red_term_app_r M N N' :
-  red_term N N' ->
-  red_term (App M N) (App M N').
-unfold red_term; intros.
-specialize H with j.
-apply Lc.redp_app_r; trivial.
-Qed.
-
-Lemma red_term_abs_l M M' N :
-  red_term M M' ->
-  red_term (Abs M N) (Abs M' N).
-unfold red_term; intros.
-specialize H with j.
-simpl.
-apply Lc.redp_app_r; trivial.
-Qed.
-
-Lemma red_term_abs_r M N N' :
-  red_term N N' ->
-  red_term (Abs M N) (Abs M N').
-unfold red_term; intros.
-specialize H with (Lc.ilift j).
-simpl.
-apply Lc.redp_app_l; trivial.
-apply Lc.redp_app_r; trivial.
-apply Lc.redp_abs; trivial.
-Qed.
-
-
-Lemma red_term_prod_l M M' N :
-  red_term M M' ->
-  red_term (Prod M N) (Prod M' N).
-unfold red_term; intros.
-specialize H with j.
-simpl.
-apply Lc.redp_app_l; trivial.
-apply Lc.redp_app_r; trivial.
-Qed.
-
-Lemma red_term_prod_r M N N' :
-  red_term N N' ->
-  red_term (Prod M N) (Prod M N').
-unfold red_term; intros.
-specialize H with (Lc.ilift j).
-simpl.
-apply Lc.redp_app_r; trivial.
-apply Lc.redp_abs; trivial.
-Qed.
-
-Lemma red1_beta T M N :
-  red_term (App (Abs T M) N) (subst N M).
-red; simpl; intros.
-eapply t_trans.
- eapply Lc.redp_app_l.
- eapply Lc.redp_K.
-
- apply t_step.
- apply Lc.red1_beta.
- unfold Lc.subst; rewrite <- tm_substitutive.
- destruct M; simpl; trivial.
- rewrite I.lams0.
- unfold I.shift; simpl.
- apply itm_morph.
- do 2 red; intros.
- destruct a; simpl.
-  rewrite Lc.lift0; trivial.
-
-  rewrite Lc.simpl_subst; auto.
-  rewrite Lc.lift0; trivial.
-Qed.
-
-Lemma red_sigma_app N A B k :
-  eq_trm (subst_rec N k (App A B)) (App (subst_rec N k A) (subst_rec N k B)).
-red; simpl; intros.
-split.
- red; intros.
- apply app_ext.
-  rewrite int_subst_rec_eq.
-  rewrite H; reflexivity.
-
-  rewrite int_subst_rec_eq.
-  rewrite H; reflexivity.
-
- red; intros.
- do 2 rewrite tm_subst_rec_eq.
- rewrite H; trivial.
-Qed.
-
-Lemma red_sigma_abs N A B k :
-  eq_trm (subst_rec N k (Abs A B)) (Abs (subst_rec N k A) (subst_rec N (S k) B)).
-red; simpl; intros.
-split.
- red; intros.
- apply lam_ext.
-  rewrite int_subst_rec_eq.
-  rewrite H; reflexivity.
-
-  red; intros.
-  rewrite int_subst_rec_eq.
-  rewrite <- V.cons_lams.
-   rewrite H1.
-   rewrite H.
-   reflexivity.
-
-   do 2 red; intros.
-   rewrite H2; reflexivity.
-
- red; intros.
- apply f_equal2.
-  apply f_equal.
-  rewrite tm_subst_rec_eq.
-  apply tm_morph; auto with *.
-  rewrite H.
-  apply Lc.cross_binder_cons.
-  unfold I.shift, Lc.ilift; simpl.
-  unfold Lc.lift; rewrite <- tm_liftable; trivial.
-
-  rewrite tm_subst_rec_eq.
-  rewrite H; auto.
-Qed.
-
-Lemma red_sigma_prod N A B k :
-  eq_trm (subst_rec N k (Prod A B)) (Prod (subst_rec N k A) (subst_rec N (S k) B)).
-red; simpl; intros.
-split.
- red; intros.
- apply prod_ext.
-  rewrite int_subst_rec_eq.
-  rewrite H; reflexivity.
-
-  red; intros.
-  rewrite int_subst_rec_eq.
-  rewrite <- V.cons_lams.
-   rewrite H1.
-   rewrite H.
-   reflexivity.
-
-   do 2 red; intros.
-   rewrite H2; reflexivity.
-
- red; intros.
- apply f_equal2.
-  rewrite tm_subst_rec_eq.
-  rewrite H; auto.
-
-  apply f_equal.
-  rewrite tm_subst_rec_eq.
-  apply tm_morph; auto with *.
-  rewrite H.
-  apply Lc.cross_binder_cons.
-  unfold I.shift, Lc.ilift; simpl.
-  unfold Lc.lift; rewrite <- tm_liftable; trivial.
-Qed.
-
-Lemma red_sigma_var_eq N k :
-  N <> kind ->
-  eq_trm (subst_rec N k (Ref k)) (lift k N).
-unfold subst_rec; simpl.
-destruct N; simpl.
-2:destruct 1; trivial.
-intros _.
-split; red; intros.
- unfold V.lams, V.shift; simpl.
- destruct (le_gt_dec k k).
- 2:omega.
- replace (k-k) with 0; auto with *.
- simpl V.cons.
- apply iint_morph.
- do 2 red; intros.
- replace (a-0) with a; auto with *.
-
- unfold I.lams; simpl.
- destruct (le_gt_dec k k).
- 2:omega.
- replace (k-k) with 0; auto with *.
- simpl I.cons.
- apply itm_morph.
- do 2 red; intros.
- unfold I.shift; simpl.
- replace (a-0) with a; auto with *.
-Qed.
-
-Lemma red_sigma_var_lt N k n :
-  n < k ->
-  eq_trm (subst_rec N k (Ref n)) (Ref n).
-unfold subst_rec; simpl; intros.
-split; red; intros.
- unfold V.lams, V.shift; simpl.
- destruct (le_gt_dec k n); auto.
- omega.
-
- unfold I.lams, I.shift; simpl.
- destruct (le_gt_dec k n); auto.
- omega.
-Qed.
-
-Lemma red_sigma_var_gt N k n :
-  k <= n ->
-  eq_trm (subst_rec N k (Ref (S n))) (Ref n).
-unfold subst_rec; simpl; intros.
-split; red; intros.
- unfold V.lams; simpl.
- destruct (le_gt_dec k (S n)); simpl.
-  unfold V.cons, V.shift; simpl.
-  destruct k; simpl; auto.
-  replace (n-k) with (S (n-S k)).
-   replace (S (k+(n- S k))) with n; auto.
-   omega.
-  omega.
- omega.
-
- unfold I.lams, I.shift, I.cons; simpl.
- destruct (le_gt_dec k (S n)); simpl.
-  destruct k; simpl; auto.
-  replace (n-k) with (S (n-S k)).
-   replace (S (k+(n- S k))) with n; auto.
-   omega.
-  omega.
- omega.
-Qed.
-
-
-Lemma simul M :
-  Lc.sn M ->
-  forall j M', M = tm j M' ->
-  Acc (transp _ red_term) M'.
-intros snM.
-Require Import Transitive_Closure.
-elim (Acc_clos_trans _ _ _ snM); clear snM; intros.
-constructor; intros.
-red in H2.
-assert (redM' := H2 j).
-assert (clos_trans _ (transp _ Lc.red1) (tm j y) x).
- rewrite H1.
- clear H1 H2.
- elim redM'; intros.
-  apply t_step; trivial.
-
-  apply t_trans with y0; trivial.
-apply H0 with (tm j y) j; trivial.
-Qed.
-
-Lemma model_strong_normalization e M T :
-  wf e ->
-  typ e M T ->
-  Acc (transp _ red_term) M.
-intros.
-destruct typ_sn with (1:=H) (2:=H0) as (j,?).
-apply simul with (1:=H1) (2:=eq_refl).
-Qed.
-
 
 End MakeModel.
 
