GenRealSN.v
@@ -43,7 +43,9 @@ Import MM.
 
 (* Derived properties of the abstract SN model *)
 
-  Notation "[ x , t ] \real A" := (x \in A  /\ inSAT t (Red A x)) (at level 60).
+(* We first introduce the realizability relation, which the conjunction
+   of the value and term interpretation requirements *)
+Notation "[ x , t ] \real A" := (x \in A  /\ inSAT t (Red A x)) (at level 60).
 
 Lemma piSAT_intro : forall A B f t,
   Lc.sn t -> (* if A is empty *)
@@ -136,428 +138,8 @@ Qed.
 
 
 (* Now the abstract strong normalization proof. *)
-
-(* Valuations *)
-Module Xeq.
-  Definition t := X.
-  Definition eq := eqX.
-  Definition eq_equiv : Equivalence eq := eqX_equiv.
-  Existing Instance eq_equiv.
-End Xeq.
-Require Import VarMap.
-Module V := VarMap.Make(Xeq).
-
-Notation val := V.map.
-Notation eq_val := V.eq_map.
-
-Definition vnil : val := V.nil props.
-
-Import V.
-Existing Instance cons_morph.
-Existing Instance cons_morph'.
-Existing Instance shift_morph.
-Existing Instance lams_morph.
-
-(* Term valuations *)
-Module I := Lambda.I.
-
-(* Terms *)
-
-Record inftrm := {
-  iint : val -> X;
-  iint_morph : Proper (eq_val ==> eqX) iint;
-  itm : Lc.intt -> Lc.term;
-  itm_morph : Proper (Lc.eq_intt ==> eq) itm;
-  itm_lift : Lc.liftable itm;
-  itm_subst : Lc.substitutive itm
-}.
-Existing Instance iint_morph.
-Existing Instance itm_morph.
-
-Definition trm := option inftrm.
-
-Definition eq_trm (x y:trm) :=
-  match x, y with
-  | Some f, Some g =>
-     (eq_val ==> eqX)%signature (iint f) (iint g) /\
-     (Lc.eq_intt ==> eq)%signature (itm f) (itm g)
-  | None, None => True
-  | _, _ => False
-  end.
-
-Instance eq_trm_refl : Reflexive eq_trm.
-red; intros.
-destruct x as [(f,mf,g,mg,sg)|]; simpl; auto.
-Qed.
-
-Instance eq_trm_sym : Symmetric eq_trm.
-red; intros.
-destruct x as [(fx,mfx,gx,mgx,sgx)|];
-destruct y as [(fy,mfy,gy,mgy,sgy)|]; simpl in *; auto.
-destruct H; split; symmetry; trivial.
-Qed.
-
-Instance eq_trm_trans : Transitive eq_trm.
-red; intros.
-destruct x as [(fx,mfx,gx,mgx,sgx)|];
-destruct y as [(fy,mfy,gy,mgy,sgy)|];
-destruct z as [(fz,mfz,gz,mgz,sgz)|];
- try contradiction; simpl in *; auto.
-destruct H; destruct H0; split.
- transitivity fy; trivial.
- transitivity gy; trivial.
-Qed.
-
-Instance eq_trm_equiv : Equivalence eq_trm.
-constructor; auto with *.
-Qed.
-
-Lemma eq_kind : forall (M:trm), M = None <-> eq_trm M None.
-destruct M; simpl; split; contradiction||discriminate||trivial.
-Qed.
-
-Definition dummy_trm : Lc.term.
-exact Lc.K.
-Defined.
-(* The only fact needed is that dummy_trm is a closed term *)
-
-Definition tm (j:Lc.intt) (M:trm) :=
-  match M with
-  | Some f => itm f j
-  | None => dummy_trm
-  end.
-
-Definition dummy_int : X.
-Proof props.
-
-Definition int (i:val) (M:trm) :=
-  match M with
-  | Some f => iint f i
-  | None => dummy_int
-  end.
-
-Lemma eq_trm_intro : forall T T',
-  (forall i, int i T == int i T') ->
-  (forall j, tm j T = tm j T') ->
-  match T, T' with Some _,Some _=>True|None,None=>True|_,_=>False end ->
-  eq_trm T T'.
-destruct T as [T|]; destruct T' as [T'|]; simpl; intros; trivial.
-split; red; intros.
- rewrite H2; auto.
- rewrite H2; auto.
-Qed.
-
-Instance tm_morph : Proper (Lc.eq_intt ==> eq_trm ==> @eq Lc.term) tm.
-unfold tm; do 3 red; intros.
-destruct x0; destruct y0; simpl in *; (contradiction||reflexivity||auto).
-destruct H0; simpl in *.
-apply H1; trivial.
-Qed.
-
-Lemma tm_substitutive : forall u t j k,
-  tm (fun n => Lc.subst_rec u (j n) k) t =
-  Lc.subst_rec u (tm j t) k.
-destruct t; simpl; intros; trivial.
-apply itm_subst.
-Qed.
-
-Lemma tm_liftable : forall j t k,
-  tm (fun n => Lc.lift_rec 1 (j n) k) t = Lc.lift_rec 1 (tm j t) k.
-destruct t; simpl; intros; trivial.
-apply itm_lift.
-Qed.
-
-Lemma tm_subst_cons : forall x j t,
-  tm (I.cons x j) t = Lc.subst x (tm (Lc.ilift j) t).
-unfold Lc.subst; intros.
-rewrite <- tm_substitutive.
-apply tm_morph; [red; intros|reflexivity].
-red.
-destruct a; simpl.
- rewrite Lc.lift0; trivial.
- rewrite Lc.simpl_subst; trivial; rewrite Lc.lift0; trivial.
-Qed.
-
-Instance int_morph : Proper (eq_val ==> eq_trm ==> eqX) int.
-unfold int; do 3 red; intros.
-destruct x0; destruct y0; simpl in *; (contradiction||reflexivity||auto).
-destruct H0; simpl in *.
-apply H0; trivial.
-Qed.
-
-Definition cst (x:X) (t:Lc.term)
-  (H0 : Lc.liftable (fun _ => t)) (H1 : Lc.substitutive (fun _ => t)) : trm.
-left; exists (fun _ => x) (fun _ => t); trivial.
- do 2 red; reflexivity.
- do 2 red; reflexivity.
-Defined.
-
-Definition kind : trm := None.
-
-Definition prop : trm := @cst props (Lc.K) (fun _ _ => eq_refl _) (fun _ _ _ => eq_refl _).
-
-Definition Ref (n:nat) : trm.
-left; exists (fun i => i n) (fun j => j n).
- do 2 red; simpl; auto.
- do 2 red; simpl; auto.
- red; reflexivity.
- red; reflexivity.
-Defined.
-
-Definition App (u v:trm) : trm.
-left; exists (fun i => app (int i u) (int i v))
-             (fun j => Lc.App (tm j u) (tm j v)). 
- do 2 red; simpl; intros.
- rewrite H; reflexivity.
-
- do 2 red; simpl; intros.
- rewrite H; reflexivity.
-
- red; simpl; intros.
- do 2 rewrite <- tm_liftable; trivial.
-
- red; simpl; intros.
- do 2 rewrite <- tm_substitutive; trivial.
-Defined.
-
-(* Church-style abstraction: *)
-Definition CAbs t m :=
-  Lc.App2 Lc.K (Lc.Abs m) t.
-
-Definition Abs (A M:trm) : trm.
-left; exists (fun i => lam (int i A) (fun x => int (V.cons x i) M))
-             (fun j => CAbs (tm j A) (tm (Lc.ilift j) M)).
- do 2 red; simpl; intros.
- apply lam_ext.
-  rewrite H; reflexivity.
-
-  red; intros.
-  rewrite H; rewrite H1; reflexivity.
-
- do 2 red; intros.
- rewrite H; trivial.
-
- red; simpl; intros.
- rewrite Lc.ilift_binder_lift; trivial.
- do 2 rewrite <- tm_liftable; trivial.
-
- red; simpl; intros.
- rewrite Lc.ilift_binder; trivial.
- do 2 rewrite <- tm_substitutive; trivial.
-Defined.
-
-(* Encoding product *)
-Definition CProd a b :=
-  Lc.App2 Lc.K a (Lc.Abs b).
-
-Definition Prod (A B:trm) : trm.
-left;
-  exists (fun i => prod (int i A) (fun x => int (V.cons x i) B))
-         (fun j => CProd (tm j A) (tm (Lc.ilift j) B)).
-do 2 red; simpl; intros.
- apply prod_ext.
-  rewrite H; reflexivity.
-
-  red; intros.
-  rewrite H; rewrite H1; reflexivity.
-
- do 2 red; intros.
- rewrite H; trivial.
-
- red; simpl; intros.
- do 2 rewrite <- tm_liftable; trivial.
- rewrite Lc.ilift_binder_lift; trivial.
-
- red; simpl; intros.
- do 2 rewrite <- tm_substitutive; trivial.
- rewrite Lc.ilift_binder; trivial.
-Defined.
-
-Lemma intProd_eq i A B :
-  int i (Prod A B) = prod (int i A) (fun x => int (V.cons x i) B).
-reflexivity.
-Qed.
-
-Definition lift_rec (n m:nat) (t:trm) : trm.
-destruct t as [t|]; [left|exact kind].
-exists (fun i => iint t (V.lams m (V.shift n) i))
-       (fun j => itm t (I.lams m (I.shift n) j)).
- do 2 red; intros.
- rewrite H; reflexivity.
-
- do 2 red; intros.
- rewrite H; reflexivity.
-
- red; intros.
- rewrite <- itm_lift.
- apply itm_morph; do 2 red; intros.
- unfold I.lams.
- destruct (le_gt_dec m a); trivial.
-
- red; intros.
- rewrite <- itm_subst.
- apply itm_morph; do 2 red; intros.
- unfold I.lams.
- destruct (le_gt_dec m a); trivial.
-Defined.
-
-Lemma int_lift_rec_eq : forall n k T i,
-  int i (lift_rec n k T) == int (V.lams k (V.shift n) i) T.
-intros; destruct T as [T|]; simpl; reflexivity.
-Qed.
-
-Definition lift n := lift_rec n 0.
-
-Instance lift_morph : forall k, Proper (eq_trm ==> eq_trm) (lift k).
-do 2 red; simpl; intros.
-destruct x as [x|]; destruct y as [y|];
-  simpl in *; (contradiction||trivial).
-destruct H; split.
- red; intros.
- apply H; rewrite H1; reflexivity.
-
- red; intros.
- apply H0; rewrite H1; reflexivity.
-Qed.
-
-Lemma int_lift_eq : forall i T,
-  int i (lift 1 T) == int (V.shift 1 i) T.
-unfold int; intros;
-  destruct T as [T|]; simpl; auto. (* BUG: intros needed before destruct *)
-2:reflexivity.
-rewrite V.lams0.
-reflexivity.
-Qed.
-
-Lemma int_cons_lift_eq : forall i T x,
-  int (V.cons x i) (lift 1 T) == int i T.
-intros.
-rewrite int_lift_eq.
-rewrite V.shift_cons; reflexivity.
-Qed.
-
-Lemma tm_lift_rec_eq : forall n k T j,
-  tm j (lift_rec n k T) = tm (I.lams k (I.shift n) j) T.
-intros; destruct T; simpl; reflexivity.
-Qed.
-
-Lemma split_lift : forall n T,
-  eq_trm (lift (S n) T) (lift 1 (lift n T)).
-destruct T as [T|]; simpl; auto.
-split; red; intros.
- do 2 rewrite V.lams0.
- change (V.shift n (fun k => V.lams 0 (V.shift 1) y k)) with
-   (V.shift n (V.lams 0 (V.shift 1) y)).
- rewrite V.lams0.
- rewrite V.shift_split.
- change (eq_val (fun k => x k) (fun k => y k)) in H.
- rewrite H; reflexivity.
-
- do 2 rewrite I.lams0.
- change (I.shift n (fun k => I.lams 0 (I.shift 1) y k)) with
-   (I.shift n (I.lams 0 (I.shift 1) y)).
- rewrite I.lams0.
- rewrite I.shift_split.
- change (Lc.eq_intt (fun k => x k) (fun k => y k)) in H.
- rewrite H; reflexivity.
-Qed.
-
-Definition subst_rec (arg:trm) (m:nat) (t:trm) : trm.
-destruct t as [body|]; [left|right].
-exists (fun i => iint body (V.lams m (V.cons (int (V.shift m i) arg)) i))
-       (fun j => itm body (I.lams m (I.cons (tm (I.shift m j) arg)) j)).
- do 2 red; intros.
- rewrite H; reflexivity.
-
- do 2 red; intros.
- rewrite H; reflexivity.
-
- red; intros.
- rewrite <- itm_lift.
- apply itm_morph; do 2 red; intros.
- unfold I.lams.
- destruct (le_gt_dec m a); trivial.
- destruct (a-m); simpl; auto.
- rewrite <- tm_liftable.
- reflexivity.
-
- red; intros.
- rewrite <- itm_subst.
- apply itm_morph; do 2 red; intros.
- unfold I.lams.
- destruct (le_gt_dec m a); trivial.
- destruct (a-m); simpl; auto.
- rewrite <- tm_substitutive.
- reflexivity.
-Defined.
-
-Lemma int_subst_rec_eq : forall arg k T i,
-  int i (subst_rec arg k T) == int (V.lams k (V.cons (int (V.shift k i) arg)) i) T.
-intros; destruct T as [T|]; simpl; reflexivity.
-Qed.
-
-Definition subst arg := subst_rec arg 0.
-
-Lemma int_subst_eq : forall N M i,
- int (V.cons (int i N) i) M == int i (subst N M).
-destruct M as [M|]; simpl; intros.
-2:reflexivity.
-rewrite V.lams0.
-rewrite V.shift0.
-reflexivity.
-Qed.
-
-Lemma tm_subst_rec_eq : forall arg k T j,
-  tm j (subst_rec arg k T) = tm (I.lams k (I.cons (tm (I.shift k j) arg)) j) T.
-intros; destruct T; simpl; reflexivity.
-Qed.
-
-Lemma tm_subst_eq : forall u v j,
-  tm j (subst u v) = Lc.subst (tm j u) (tm (Lc.ilift j) v).
-intros.
-unfold Lc.subst; rewrite <- tm_substitutive.
-destruct v as [v|]; simpl; trivial.
-rewrite I.lams0.
-rewrite I.shift0.
-apply itm_morph.
-apply I.cons_ext; simpl.
- rewrite Lc.lift0; trivial.
-
- do 2 red; unfold I.shift; simpl; intros.
- rewrite Lc.simpl_subst; trivial; rewrite Lc.lift0; trivial.
-Qed.
-
-Instance App_morph : Proper (eq_trm ==> eq_trm ==> eq_trm) App.
-unfold App; do 3 red; simpl; split; intros.
- red; intros.
- rewrite H; rewrite H0; rewrite H1; reflexivity.
-
- red; intros.
- rewrite H; rewrite H0; rewrite H1; reflexivity.
-Qed.
-
-Instance Abs_morph : Proper (eq_trm ==> eq_trm ==> eq_trm) Abs.
-unfold Abs; do 4 red; simpl; split; red; intros.
- apply lam_ext.
-  apply int_morph; auto.
-
-  red; intros.
-  rewrite H0; rewrite H1; rewrite H3; reflexivity.
-
- rewrite H0; rewrite H1; rewrite H; reflexivity.
-Qed.
-
-
-Instance Prod_morph : Proper (eq_trm ==> eq_trm ==> eq_trm) Prod.
-unfold Prod; do 4 red; simpl; split; red; intros.
- apply prod_ext.
-  rewrite H; rewrite H1; reflexivity.
-
-  red; intros.
-  rewrite H0; rewrite H1; rewrite H3; reflexivity.
-
- rewrite H0; rewrite H1; rewrite H; reflexivity.
-Qed.
+Require ObjectSN.
+Include ObjectSN.MakeObject(M).
 
 
 (* Dealing with top sorts.
@@ -581,12 +163,6 @@ apply lam_ext; intros.
  apply IHx0.
  rewrite H2; rewrite H; reflexivity.
 Qed.
-
-Fixpoint prod_list (e:list trm) (U:trm) :=
-  match e with
-  | List.nil => U
-  | T::f => Prod T (prod_list f U)
-  end.
 
 Fixpoint cst_trm (e:list trm) (x:Lc.term) : Lc.term :=
   match e with
@@ -671,45 +247,36 @@ rewrite eq_U.
 apply wit_prod; trivial.
 Qed.
 
-Lemma discr_ref_prod : forall n A B,
-  ~ eq_trm (Ref n) (Prod A B).
-red; intros.
-simpl in H.
-destruct H as (_,H).
-red in H.
-specialize H with Lc.Ref Lc.Ref.
-discriminate H.
-reflexivity.
-Qed.
-
-Lemma lift1var : forall n, eq_trm (lift 1 (Ref n)) (Ref (S n)).
-simpl; split; red; intros.
- revert n.
- change (eq_val (V.lams 0 (V.shift 1) x) (V.shift 1 y)).
- rewrite V.lams0; rewrite <- H.
- reflexivity.
-
- revert n.
- change (Lc.eq_intt (I.lams 0 (I.shift 1) x) (I.shift 1 y)).
- rewrite I.lams0; rewrite <- H.
- reflexivity.
-Qed.
-
-Lemma non_empty_var_lift : forall n,
-  non_empty (Ref n) -> non_empty (Ref (S n)).
-intros n (e,(U,eq_U,(x,(t,in_U)))).
-destruct e; simpl prod_list in eq_U.
- exists List.nil; exists (lift 1 U).
-  simpl prod_list.
-  rewrite <- lift1var.
-  apply lift_morph; trivial.
+Lemma non_empty_lift M k :
+  non_empty M <-> non_empty (lift_rec 1 k M).
+unfold non_empty; split; intros.
+ destruct H as (e,(U,?,(x,(t,?)))).
+ destruct lift_prod_list_ex with 1 k e U as (e',?).
+ exists e'.
+ exists (lift_rec 1 (length e+k) U).
+  rewrite H; trivial.
 
   exists x; exists t; intros.
-  rewrite int_lift_eq; auto.
+  rewrite int_lift_rec_eq.
+  apply H0.
 
- elim (discr_ref_prod eq_U).
+ destruct H as (e,(U,?,(x,(t,?)))).
+ destruct subst_prod_list_ex with (Ref 0) k e U as (e',?).
+ exists e'.
+ exists (subst_rec (Ref 0) (length e+k) U).
+  rewrite <- H1.
+  rewrite <- H.
+  apply simpl_subst_lift_rec.
+
+  exists x; exists t; intros.
+  rewrite int_subst_rec_eq.
+  apply H0.
 Qed.
 
+(* Semantic typing relation.
+   Handles the case of kind: a type that contains all "non-empty" types
+   and that is included in no type.
+ *)
 
 Definition in_int (i:val) (j:Lc.intt) (M T:trm) :=
   M <> None /\
@@ -777,7 +344,8 @@ split; try discriminate.
   rewrite int_cons_lift_eq; trivial.
 
   destruct mem; split; trivial.
-  apply non_empty_var_lift; trivial.
+  rewrite non_empty_lift with (k:=0) in H.
+  rewrite eq_trm_lift_ref_fv in H; auto with arith.
 Qed.
 
 Lemma in_int_sn : forall i j M T,
@@ -915,15 +483,26 @@ destruct 1 as [ty_T|ty_T]; intro is_val; apply ty_T in is_val;
  destruct is_val as (_,mem); apply real_sn in mem; trivial.
 Qed.
 
-Lemma typ_sn : forall e M T,
-  wf e -> typ e M T -> exists j, Lc.sn (tm j M).
-intros e M T (i,(j,is_val)) ty.
-exists j.
+(* This lemma shows that the abstract model construction entails
+   strong normalization.
+   At this level, we do have the actual syntax. However, red_term
+   is a relation on the denotations that admits the same introduction
+   rules as the syntactic reduction.
+   When the syntax is introduced, it will only remain to check that
+   the syntactic reduction implies the semantic one, which will be
+   straightforward.
+ *)
+Lemma model_strong_normalization e M T :
+  wf e ->
+  typ e M T ->
+  Acc (transp _ red_term) M.
+intros (i,(j,is_val)) ty.
 apply ty in is_val.
-apply in_int_sn in is_val; trivial.
+apply in_int_sn in is_val.
+apply simul with (1:=is_val) (2:=eq_refl).
 Qed.
 
-(* Context formation *)
+(* Context formation rules *)
 
 Lemma wf_nil : wf List.nil.
 red.
@@ -955,7 +534,8 @@ Lemma sym : forall e M M', eq_typ e M M' -> eq_typ e M' M.
 unfold eq_typ; destruct 1; split; intros; symmetry; eauto.
 Qed.
 
-Lemma trans : forall e M M' M'', eq_typ e M M' -> eq_typ e M' M'' -> eq_typ e M M''.
+Lemma trans : forall e M M' M'',
+  eq_typ e M M' -> eq_typ e M' M'' -> eq_typ e M M''.
 unfold eq_typ; destruct 1; destruct 1; split; intros.
  transitivity (int i M'); eauto.
 
@@ -1090,7 +670,6 @@ red; simpl; intros.
 apply H0 in H; trivial.
 Qed.
 
-
 Lemma typ_app : forall e u v V Ur,
   typ e v V ->
   typ e u (Prod V Ur) ->
@@ -1209,7 +788,7 @@ destruct is_srt; subst s2; simpl in *.
  unfold CProd.
  apply real_exp_K.
   apply Lc.sn_abs; trivial.
- assert (prod (int i T) (fun x => int (cons x i) U) \in props).
+ assert (prod (int i T) (fun x => int (V.cons x i) U) \in props).
   apply impredicative_prod; intros.   
    red; intros.
    rewrite H1; reflexivity.
@@ -1243,27 +822,41 @@ Qed.
 
 (* Weakening *)
 
-(*
+
 Lemma weakening : forall e M T A,
   typ e M T ->
   typ (A::e) (lift 1 M) (lift 1 T).
 unfold typ, in_int; intros.
-destruct T as [(T,Tm)|]; simpl in *; trivial.
-red; simpl.
-unfold lift.
-rewrite int_lift_rec_eq.
-apply H.
-unfold val_ok in *.
-intros.
-specialize (H0 (S n) _ H1).
-destruct T0 as [(T0,T0m)|]; simpl in *; trivial.
-unfold V.lams at 1, V.shift at 1 2; simpl.
-replace (n-0) with n; auto with arith.
+assert (val_ok e (V.lams 0 (V.shift 1) i) (I.lams 0 (I.shift 1) j)).
+ red; intros.
+ rewrite I.lams0; rewrite V.lams0; unfold V.shift, I.shift; simpl.
+ red in H0.
+ apply H0 with (n:=S n) in H1.
+ revert H1.
+ unfold in_int; destruct T0 as [(T0,T0m)|]; simpl.
+  intros (_,realV); split;[discriminate|exact realV].
+
+  intros (_,(ne,sat)); split;[discriminate|split; trivial].
+
+  rewrite non_empty_lift with (k:=0).
+  rewrite eq_trm_lift_ref_fv; auto with *.
+destruct H with (1:=H1) as (M_nk, inT).
+split.
+ destruct M; try discriminate.
+ elim M_nk; trivial.
+ revert inT; pattern T at 1 4; case T; intros; simpl.
+ unfold lift.
+ do 2 rewrite int_lift_rec_eq.
+ rewrite tm_lift_rec_eq; trivial.
+
+ destruct inT; split.
+  unfold lift; rewrite <- non_empty_lift; trivial.
+
+  unfold lift; rewrite tm_lift_rec_eq; trivial.
 Qed.
-*)
 
 
-(* Subtyping *)
+(* Subtyping rules *)
 
 Lemma sub_refl : forall e M M',
   eq_typ e M M' -> sub_typ e M M'.
@@ -1296,359 +889,49 @@ destruct T' as [(T',T'm)|]; simpl in *; trivial; auto.
  elim H2; trivial.
 Qed.
 
-(* "Untyped" reduction: tools for proving simulation and strong normalization *)
+(* Covariance can be derived if we have a weak eta property:
+   any function is a lambda abstraction *with the same domain*.
+   This is OK with set-theoretical functions (in contrast with
+   general eta which does not hold on set-theoretical functions).
+   This property could be added to the abstract domain.
 
-Require Import Relations.
-
-Definition red_term M N :=
-  forall j, Lc.redp (tm j M) (tm j N).
-
-Instance red_term_morph : Proper (eq_trm ==> eq_trm ==> iff) red_term.
-apply morph_impl_iff2; auto with *.
-do 4 red; intros.
-red; intros.
-rewrite <- H; rewrite <- H0; auto.
-Qed.
-
-Lemma red_term_trans M1 M2 M3 :
-  red_term M1 M2 -> red_term M2 M3 -> red_term M1 M3.
-unfold red_term; intros.
-specialize H with j.
-specialize H0 with j.
-apply t_trans with (tm j M2); trivial.
-Qed.
-
-Lemma red_term_app_l M M' N :
-  red_term M M' ->
-  red_term (App M N) (App M' N).
-unfold red_term; intros.
-specialize H with j.
-apply Lc.redp_app_l; trivial.
-Qed.
-
-Lemma red_term_app_r M N N' :
-  red_term N N' ->
-  red_term (App M N) (App M N').
-unfold red_term; intros.
-specialize H with j.
-apply Lc.redp_app_r; trivial.
-Qed.
-
-Lemma red_term_abs_l M M' N :
-  red_term M M' ->
-  red_term (Abs M N) (Abs M' N).
-unfold red_term; intros.
-specialize H with j.
-simpl.
-apply Lc.redp_app_r; trivial.
-Qed.
-
-Lemma red_term_abs_r M N N' :
-  red_term N N' ->
-  red_term (Abs M N) (Abs M N').
-unfold red_term; intros.
-specialize H with (Lc.ilift j).
-simpl.
-apply Lc.redp_app_l; trivial.
-apply Lc.redp_app_r; trivial.
-apply Lc.redp_abs; trivial.
-Qed.
-
-Lemma red_term_prod_l M M' N :
-  red_term M M' ->
-  red_term (Prod M N) (Prod M' N).
-unfold red_term; intros.
-specialize H with j.
-simpl.
-apply Lc.redp_app_l; trivial.
-apply Lc.redp_app_r; trivial.
-Qed.
-
-Lemma red_term_prod_r M N N' :
-  red_term N N' ->
-  red_term (Prod M N) (Prod M N').
-unfold red_term; intros.
-specialize H with (Lc.ilift j).
-simpl.
-apply Lc.redp_app_r; trivial.
-apply Lc.redp_abs; trivial.
-Qed.
-
-Lemma red_term_beta T M N :
-  red_term (App (Abs T M) N) (subst N M).
-red; simpl; intros.
-eapply t_trans.
- eapply Lc.redp_app_l.
- eapply Lc.redp_K.
-
- apply t_step.
- apply Lc.red1_beta.
- unfold Lc.subst; rewrite <- tm_substitutive.
- destruct M; simpl; trivial.
- rewrite I.lams0.
- unfold I.shift; simpl.
- apply itm_morph.
- do 2 red; intros.
- destruct a; simpl.
-  rewrite Lc.lift0; trivial.
-
-  rewrite Lc.simpl_subst; auto.
-  rewrite Lc.lift0; trivial.
-Qed.
-
-Lemma red_lift_app n A B k :
-  eq_trm (lift_rec n k (App A B)) (App (lift_rec n k A) (lift_rec n k B)).
-red; simpl; intros.
-split.
- red; intros.
- apply app_ext.
-  rewrite int_lift_rec_eq.
-  rewrite H; reflexivity.
-
-  rewrite int_lift_rec_eq.
-  rewrite H; reflexivity.
-
- red; intros.
- do 2 rewrite tm_lift_rec_eq.
- rewrite H; trivial.
-Qed.
-
-Lemma red_lift_abs n A B k :
-  eq_trm (lift_rec n k (Abs A B)) (Abs (lift_rec n k A) (lift_rec n (S k) B)).
-red; simpl; intros.
-split.
- red; intros.
+   Contravariance of product does not hold in set-theory.
+ *)
+Definition sub_typ_covariant
+  (eta_eq : forall dom F f, f \in prod dom F -> f == lam dom (app f))
+  e U1 U2 V1 V2 :
+  U1 <> kind ->
+  eq_typ e U1 U2 ->
+  sub_typ (U1::e) V1 V2 ->
+  sub_typ e (Prod U1 V1) (Prod U2 V2).
+unfold sub_typ; simpl; intros U1_nk eqU subV i j is_val x t in1.
+assert (eqx : x == lam (int i U2) (app x)).
+ destruct in1 as (tyx,_).
+ apply eta_eq in tyx.
+ apply (transitivity tyx).
  apply lam_ext.
-  rewrite int_lift_rec_eq.
-  rewrite H; reflexivity.
+  apply (proj1 eqU) with (1:=is_val).
 
-  red; intros.
-  rewrite int_lift_rec_eq.
-  rewrite <- V.cons_lams.
-   rewrite H1.
-   rewrite H.
-   reflexivity.
-
-   do 2 red; intros.
-   rewrite H2; reflexivity.
+  red; intros; apply app_ext; auto with *.
+rewrite eqx.
+apply prod_intro_sn.
+ red; intros; apply app_ext; auto with *.
 
  red; intros.
- apply f_equal2.
-  rewrite tm_lift_rec_eq.
-  rewrite H; auto.
+ rewrite H0; reflexivity.
 
-  rewrite tm_lift_rec_eq.
-  apply tm_morph; auto with *.
-  rewrite H.
-  apply Lc.cross_binder_shift.
-Qed.
+ apply real_sn in in1; trivial.
 
-Lemma red_lift_prod n A B k :
-  eq_trm (lift_rec n k (Prod A B)) (Prod (lift_rec n k A) (lift_rec n (S k) B)).
-red; simpl; intros.
-split.
- red; intros.
- apply prod_ext.
-  rewrite int_lift_rec_eq.
-  rewrite H; reflexivity.
+ intros.
+ apply subV with (j:=I.cons u j).
+  apply vcons_add_var; trivial.
+  rewrite (proj1 eqU _ _ is_val); trivial.
 
-  red; intros.
-  rewrite int_lift_rec_eq.
-  rewrite <- V.cons_lams.
-   rewrite H1.
-   rewrite H.
-   reflexivity.
+  apply prod_elim with (2:=in1).
+   red; intros.
+   rewrite H1; auto with *.
 
-   do 2 red; intros.
-   rewrite H2; reflexivity.
-
- red; intros.
- apply f_equal2.
-  rewrite tm_lift_rec_eq.
-  rewrite H; auto.
-
-  rewrite tm_lift_rec_eq.
-  apply tm_morph; auto with *.
-  rewrite H.
-  apply Lc.cross_binder_shift.
-Qed.
-
-Lemma red_sigma_app N A B k :
-  eq_trm (subst_rec N k (App A B)) (App (subst_rec N k A) (subst_rec N k B)).
-red; simpl; intros.
-split.
- red; intros.
- apply app_ext.
-  rewrite int_subst_rec_eq.
-  rewrite H; reflexivity.
-
-  rewrite int_subst_rec_eq.
-  rewrite H; reflexivity.
-
- red; intros.
- do 2 rewrite tm_subst_rec_eq.
- rewrite H; trivial.
-Qed.
-
-Lemma red_sigma_abs N A B k :
-  eq_trm (subst_rec N k (Abs A B)) (Abs (subst_rec N k A) (subst_rec N (S k) B)).
-red; simpl; intros.
-split.
- red; intros.
- apply lam_ext.
-  rewrite int_subst_rec_eq.
-  rewrite H; reflexivity.
-
-  red; intros.
-  rewrite int_subst_rec_eq.
-  rewrite <- V.cons_lams.
-   rewrite H1.
-   rewrite H.
-   reflexivity.
-
-   do 2 red; intros.
-   rewrite H2; reflexivity.
-
- red; intros.
- apply f_equal2.
-  rewrite tm_subst_rec_eq.
-  rewrite H; auto.
-
-  rewrite tm_subst_rec_eq.
-  apply tm_morph; auto with *.
-  rewrite H.
-  apply Lc.cross_binder_cons.
-  unfold I.shift, Lc.ilift; simpl.
-  unfold Lc.lift; rewrite <- tm_liftable; trivial.
-Qed.
-
-Lemma red_sigma_prod N A B k :
-  eq_trm (subst_rec N k (Prod A B)) (Prod (subst_rec N k A) (subst_rec N (S k) B)).
-red; simpl; intros.
-split.
- red; intros.
- apply prod_ext.
-  rewrite int_subst_rec_eq.
-  rewrite H; reflexivity.
-
-  red; intros.
-  rewrite int_subst_rec_eq.
-  rewrite <- V.cons_lams.
-   rewrite H1.
-   rewrite H.
-   reflexivity.
-
-   do 2 red; intros.
-   rewrite H2; reflexivity.
-
- red; intros.
- apply f_equal2.
-  rewrite tm_subst_rec_eq.
-  rewrite H; auto.
-
-  rewrite tm_subst_rec_eq.
-  apply tm_morph; auto with *.
-  rewrite H.
-  apply Lc.cross_binder_cons.
-  unfold I.shift, Lc.ilift; simpl.
-  unfold Lc.lift; rewrite <- tm_liftable; trivial.
-Qed.
-
-Lemma red_sigma_var_eq N k :
-  N <> kind ->
-  eq_trm (subst_rec N k (Ref k)) (lift k N).
-unfold subst_rec; simpl.
-destruct N; simpl.
-2:destruct 1; trivial.
-intros _.
-split; red; intros.
- unfold V.lams, V.shift; simpl.
- destruct (le_gt_dec k k).
- 2:omega.
- replace (k-k) with 0; auto with *.
- simpl V.cons.
- apply iint_morph.
- do 2 red; intros.
- replace (a-0) with a; auto with *.
-
- unfold I.lams; simpl.
- destruct (le_gt_dec k k).
- 2:omega.
- replace (k-k) with 0; auto with *.
- simpl I.cons.
- apply itm_morph.
- do 2 red; intros.
- unfold I.shift; simpl.
- replace (a-0) with a; auto with *.
-Qed.
-
-Lemma red_sigma_var_lt N k n :
-  n < k ->
-  eq_trm (subst_rec N k (Ref n)) (Ref n).
-unfold subst_rec; simpl; intros.
-split; red; intros.
- unfold V.lams, V.shift; simpl.
- destruct (le_gt_dec k n); auto.
- omega.
-
- unfold I.lams, I.shift; simpl.
- destruct (le_gt_dec k n); auto.
- omega.
-Qed.
-
-Lemma red_sigma_var_gt N k n :
-  k <= n ->
-  eq_trm (subst_rec N k (Ref (S n))) (Ref n).
-unfold subst_rec; simpl; intros.
-split; red; intros.
- unfold V.lams; simpl.
- destruct (le_gt_dec k (S n)); simpl.
-  unfold V.cons, V.shift; simpl.
-  destruct k; simpl; auto.
-  replace (n-k) with (S (n-S k)).
-   replace (S (k+(n- S k))) with n; auto.
-   omega.
-  omega.
- omega.
-
- unfold I.lams, I.shift, I.cons; simpl.
- destruct (le_gt_dec k (S n)); simpl.
-  destruct k; simpl; auto.
-  replace (n-k) with (S (n-S k)).
-   replace (S (k+(n- S k))) with n; auto.
-   omega.
-  omega.
- omega.
-Qed.
-
-Require Import Transitive_Closure.
-
-Lemma simul M :
-  Lc.sn M ->
-  forall j M', M = tm j M' ->
-  Acc (transp _ red_term) M'.
-intros snM.
-elim (Acc_clos_trans _ _ _ snM); clear snM; intros.
-constructor; intros.
-red in H2.
-assert (redM' := H2 j).
-assert (clos_trans _ (transp _ Lc.red1) (tm j y) x).
- rewrite H1.
- clear H1 H2.
- elim redM'; intros.
-  apply t_step; trivial.
-
-  apply t_trans with y0; trivial.
-apply H0 with (tm j y) j; trivial.
-Qed.
-
-Lemma model_strong_normalization e M T :
-  wf e ->
-  typ e M T ->
-  Acc (transp _ red_term) M.
-intros.
-destruct typ_sn with (1:=H) (2:=H0) as (j,?).
-apply simul with (1:=H1) (2:=eq_refl).
+   rewrite (proj1 eqU _ _ is_val); trivial.
 Qed.
 
 End MakeModel.
