ObjectSN.v
@@ -1,0 +1,920 @@
+Require Export basic.
+Require Import Models.
+Require Import VarMap.
+Require Lambda.
+Module Lc := Lambda.
+
+Module MakeObject (M: CC_Model).
+Import M.
+
+(* Valuations *)
+Module Xeq.
+  Definition t := X.
+  Definition eq := eqX.
+  Definition eq_equiv : Equivalence eq := eqX_equiv.
+  Existing Instance eq_equiv.
+End Xeq.
+Module V := VarMap.Make(Xeq).
+
+Notation val := V.map.
+Notation eq_val := V.eq_map.
+
+Definition vnil : val := V.nil props.
+
+Existing Instance V.cons_morph.
+Existing Instance V.cons_morph'.
+Existing Instance V.shift_morph.
+Existing Instance V.lams_morph.
+
+(* Term valuations *)
+Module I := Lambda.I.
+
+(* Terms *)
+
+Record inftrm := {
+  iint : val -> X;
+  iint_morph : Proper (eq_val ==> eqX) iint;
+  itm : Lc.intt -> Lc.term;
+  itm_morph : Proper (Lc.eq_intt ==> eq) itm;
+  itm_lift : Lc.liftable itm;
+  itm_subst : Lc.substitutive itm
+}.
+Existing Instance iint_morph.
+Existing Instance itm_morph.
+
+Definition trm := option inftrm.
+
+Definition eq_trm (x y:trm) :=
+  match x, y with
+  | Some f, Some g =>
+     (eq_val ==> eqX)%signature (iint f) (iint g) /\
+     (Lc.eq_intt ==> eq)%signature (itm f) (itm g)
+  | None, None => True
+  | _, _ => False
+  end.
+
+Instance eq_trm_refl : Reflexive eq_trm.
+red; intros.
+destruct x as [(f,mf,g,mg,sg)|]; simpl; auto.
+Qed.
+
+Instance eq_trm_sym : Symmetric eq_trm.
+red; intros.
+destruct x as [(fx,mfx,gx,mgx,sgx)|];
+destruct y as [(fy,mfy,gy,mgy,sgy)|]; simpl in *; auto.
+destruct H; split; symmetry; trivial.
+Qed.
+
+Instance eq_trm_trans : Transitive eq_trm.
+red; intros.
+destruct x as [(fx,mfx,gx,mgx,sgx)|];
+destruct y as [(fy,mfy,gy,mgy,sgy)|];
+destruct z as [(fz,mfz,gz,mgz,sgz)|];
+ try contradiction; simpl in *; auto.
+destruct H; destruct H0; split.
+ transitivity fy; trivial.
+ transitivity gy; trivial.
+Qed.
+
+Instance eq_trm_equiv : Equivalence eq_trm.
+constructor; auto with *.
+Qed.
+
+Lemma eq_kind : forall (M:trm), M = None <-> eq_trm M None.
+destruct M; simpl; split; contradiction||discriminate||trivial.
+Qed.
+
+Definition dummy_trm : Lc.term.
+exact Lc.K.
+Defined.
+(* The only fact needed is that dummy_trm is a closed term *)
+
+Definition tm (j:Lc.intt) (M:trm) :=
+  match M with
+  | Some f => itm f j
+  | None => dummy_trm
+  end.
+
+Definition dummy_int : X.
+Proof props.
+
+Definition int (i:val) (M:trm) :=
+  match M with
+  | Some f => iint f i
+  | None => dummy_int
+  end.
+
+Lemma eq_trm_intro : forall T T',
+  (forall i, int i T == int i T') ->
+  (forall j, tm j T = tm j T') ->
+  match T, T' with Some _,Some _=>True|None,None=>True|_,_=>False end ->
+  eq_trm T T'.
+destruct T as [T|]; destruct T' as [T'|]; simpl; intros; trivial.
+split; red; intros.
+ rewrite H2; auto.
+ rewrite H2; auto.
+Qed.
+
+Instance tm_morph : Proper (Lc.eq_intt ==> eq_trm ==> @eq Lc.term) tm.
+unfold tm; do 3 red; intros.
+destruct x0; destruct y0; simpl in *; (contradiction||reflexivity||auto).
+destruct H0; simpl in *.
+apply H1; trivial.
+Qed.
+
+Lemma tm_substitutive : forall u t j k,
+  tm (fun n => Lc.subst_rec u (j n) k) t =
+  Lc.subst_rec u (tm j t) k.
+destruct t; simpl; intros; trivial.
+apply itm_subst.
+Qed.
+
+Lemma tm_liftable : forall j t k,
+  tm (fun n => Lc.lift_rec 1 (j n) k) t = Lc.lift_rec 1 (tm j t) k.
+destruct t; simpl; intros; trivial.
+apply itm_lift.
+Qed.
+
+Lemma tm_subst_cons : forall x j t,
+  tm (I.cons x j) t = Lc.subst x (tm (Lc.ilift j) t).
+unfold Lc.subst; intros.
+rewrite <- tm_substitutive.
+apply tm_morph; [red; intros|reflexivity].
+red.
+destruct a; simpl.
+ rewrite Lc.lift0; trivial.
+ rewrite Lc.simpl_subst; trivial; rewrite Lc.lift0; trivial.
+Qed.
+
+Instance int_morph : Proper (eq_val ==> eq_trm ==> eqX) int.
+unfold int; do 3 red; intros.
+destruct x0; destruct y0; simpl in *; (contradiction||reflexivity||auto).
+destruct H0; simpl in *.
+apply H0; trivial.
+Qed.
+
+Definition cst (x:X) (t:Lc.term)
+  (H0 : Lc.liftable (fun _ => t)) (H1 : Lc.substitutive (fun _ => t)) : trm.
+left; exists (fun _ => x) (fun _ => t); trivial.
+ do 2 red; reflexivity.
+ do 2 red; reflexivity.
+Defined.
+
+Definition kind : trm := None.
+
+Definition prop : trm :=
+  @cst props (Lc.K) (fun _ _ => eq_refl _) (fun _ _ _ => eq_refl _).
+
+Definition Ref (n:nat) : trm.
+left; exists (fun i => i n) (fun j => j n).
+ do 2 red; simpl; auto.
+ do 2 red; simpl; auto.
+ red; reflexivity.
+ red; reflexivity.
+Defined.
+
+Definition App (u v:trm) : trm.
+left; exists (fun i => app (int i u) (int i v))
+             (fun j => Lc.App (tm j u) (tm j v)). 
+ do 2 red; simpl; intros.
+ rewrite H; reflexivity.
+
+ do 2 red; simpl; intros.
+ rewrite H; reflexivity.
+
+ red; simpl; intros.
+ do 2 rewrite <- tm_liftable; trivial.
+
+ red; simpl; intros.
+ do 2 rewrite <- tm_substitutive; trivial.
+Defined.
+
+(* Church-style abstraction: *)
+Definition CAbs t m :=
+  Lc.App2 Lc.K (Lc.Abs m) t.
+
+Definition Abs (A M:trm) : trm.
+left; exists (fun i => lam (int i A) (fun x => int (V.cons x i) M))
+             (fun j => CAbs (tm j A) (tm (Lc.ilift j) M)).
+ do 2 red; simpl; intros.
+ apply lam_ext.
+  rewrite H; reflexivity.
+
+  red; intros.
+  rewrite H; rewrite H1; reflexivity.
+
+ do 2 red; intros.
+ rewrite H; trivial.
+
+ red; simpl; intros.
+ rewrite Lc.ilift_binder_lift; trivial.
+ do 2 rewrite <- tm_liftable; trivial.
+
+ red; simpl; intros.
+ rewrite Lc.ilift_binder; trivial.
+ do 2 rewrite <- tm_substitutive; trivial.
+Defined.
+
+(* Encoding product *)
+Definition CProd a b :=
+  Lc.App2 Lc.K a (Lc.Abs b).
+
+Definition Prod (A B:trm) : trm.
+left;
+  exists (fun i => prod (int i A) (fun x => int (V.cons x i) B))
+         (fun j => CProd (tm j A) (tm (Lc.ilift j) B)).
+do 2 red; simpl; intros.
+ apply prod_ext.
+  rewrite H; reflexivity.
+
+  red; intros.
+  rewrite H; rewrite H1; reflexivity.
+
+ do 2 red; intros.
+ rewrite H; trivial.
+
+ red; simpl; intros.
+ do 2 rewrite <- tm_liftable; trivial.
+ rewrite Lc.ilift_binder_lift; trivial.
+
+ red; simpl; intros.
+ do 2 rewrite <- tm_substitutive; trivial.
+ rewrite Lc.ilift_binder; trivial.
+Defined.
+
+Lemma intProd_eq i A B :
+  int i (Prod A B) = prod (int i A) (fun x => int (V.cons x i) B).
+reflexivity.
+Qed.
+
+Definition lift_rec (n m:nat) (t:trm) : trm.
+destruct t as [t|]; [left|exact kind].
+exists (fun i => iint t (V.lams m (V.shift n) i))
+       (fun j => itm t (I.lams m (I.shift n) j)).
+ do 2 red; intros.
+ rewrite H; reflexivity.
+
+ do 2 red; intros.
+ rewrite H; reflexivity.
+
+ red; intros.
+ rewrite <- itm_lift.
+ apply itm_morph; do 2 red; intros.
+ unfold I.lams.
+ destruct (le_gt_dec m a); trivial.
+
+ red; intros.
+ rewrite <- itm_subst.
+ apply itm_morph; do 2 red; intros.
+ unfold I.lams.
+ destruct (le_gt_dec m a); trivial.
+Defined.
+
+Instance lift_rec_morph n k :
+  Proper (eq_trm ==> eq_trm) (lift_rec n k).
+ do 2 red; intros.
+ destruct x; destruct y; try contradiction; try exact I.
+ red; simpl.
+ destruct H.
+ split; red; intros.
+  apply H.
+  rewrite H1; reflexivity.
+
+  apply H0.
+  rewrite H1; reflexivity.
+Qed.
+
+Lemma int_lift_rec_eq : forall n k T i,
+  int i (lift_rec n k T) == int (V.lams k (V.shift n) i) T.
+intros; destruct T as [T|]; simpl; reflexivity.
+Qed.
+
+Definition lift n := lift_rec n 0.
+
+Instance lift_morph : forall k, Proper (eq_trm ==> eq_trm) (lift k).
+do 2 red; simpl; intros.
+destruct x as [x|]; destruct y as [y|];
+  simpl in *; (contradiction||trivial).
+destruct H; split.
+ red; intros.
+ apply H; rewrite H1; reflexivity.
+
+ red; intros.
+ apply H0; rewrite H1; reflexivity.
+Qed.
+
+Lemma int_lift_eq : forall i T,
+  int i (lift 1 T) == int (V.shift 1 i) T.
+unfold int; intros;
+  destruct T as [T|]; simpl; auto. (* BUG: intros needed before destruct *)
+2:reflexivity.
+rewrite V.lams0.
+reflexivity.
+Qed.
+
+Lemma int_cons_lift_eq : forall i T x,
+  int (V.cons x i) (lift 1 T) == int i T.
+intros.
+rewrite int_lift_eq.
+rewrite V.shift_cons; reflexivity.
+Qed.
+
+Lemma tm_lift_rec_eq : forall n k T j,
+  tm j (lift_rec n k T) = tm (I.lams k (I.shift n) j) T.
+intros; destruct T; simpl; reflexivity.
+Qed.
+
+Lemma split_lift : forall n T,
+  eq_trm (lift (S n) T) (lift 1 (lift n T)).
+destruct T as [T|]; simpl; auto.
+split; red; intros.
+ do 2 rewrite V.lams0.
+ change (V.shift n (fun k => V.lams 0 (V.shift 1) y k)) with
+   (V.shift n (V.lams 0 (V.shift 1) y)).
+ rewrite V.lams0.
+ rewrite V.shift_split.
+ change (eq_val (fun k => x k) (fun k => y k)) in H.
+ rewrite H; reflexivity.
+
+ do 2 rewrite I.lams0.
+ change (I.shift n (fun k => I.lams 0 (I.shift 1) y k)) with
+   (I.shift n (I.lams 0 (I.shift 1) y)).
+ rewrite I.lams0.
+ rewrite I.shift_split.
+ change (Lc.eq_intt (fun k => x k) (fun k => y k)) in H.
+ rewrite H; reflexivity.
+Qed.
+
+Definition subst_rec (arg:trm) (m:nat) (t:trm) : trm.
+destruct t as [body|]; [left|right].
+exists (fun i => iint body (V.lams m (V.cons (int (V.shift m i) arg)) i))
+       (fun j => itm body (I.lams m (I.cons (tm (I.shift m j) arg)) j)).
+ do 2 red; intros.
+ rewrite H; reflexivity.
+
+ do 2 red; intros.
+ rewrite H; reflexivity.
+
+ red; intros.
+ rewrite <- itm_lift.
+ apply itm_morph; do 2 red; intros.
+ unfold I.lams.
+ destruct (le_gt_dec m a); trivial.
+ destruct (a-m); simpl; auto.
+ rewrite <- tm_liftable.
+ reflexivity.
+
+ red; intros.
+ rewrite <- itm_subst.
+ apply itm_morph; do 2 red; intros.
+ unfold I.lams.
+ destruct (le_gt_dec m a); trivial.
+ destruct (a-m); simpl; auto.
+ rewrite <- tm_substitutive.
+ reflexivity.
+Defined.
+
+Instance subst_rec_morph :
+  Proper (eq_trm ==> eq ==> eq_trm ==> eq_trm) subst_rec.
+do 4 red; intros.
+subst y0; rename x0 into k.
+destruct x1; destruct y1; try contradiction; try exact I.
+red; simpl.
+destruct H1.
+split; red; intros.
+ apply H0.
+ rewrite H; rewrite H2; reflexivity.
+
+ apply H1.
+ rewrite H; rewrite H2; reflexivity.
+Qed.
+
+Lemma int_subst_rec_eq : forall arg k T i,
+  int i (subst_rec arg k T) == int (V.lams k (V.cons (int (V.shift k i) arg)) i) T.
+intros; destruct T as [T|]; simpl; reflexivity.
+Qed.
+
+Definition subst arg := subst_rec arg 0.
+
+Lemma int_subst_eq : forall N M i,
+ int (V.cons (int i N) i) M == int i (subst N M).
+destruct M as [M|]; simpl; intros.
+2:reflexivity.
+rewrite V.lams0.
+rewrite V.shift0.
+reflexivity.
+Qed.
+
+Lemma tm_subst_rec_eq : forall arg k T j,
+  tm j (subst_rec arg k T) = tm (I.lams k (I.cons (tm (I.shift k j) arg)) j) T.
+intros; destruct T; simpl; reflexivity.
+Qed.
+
+Lemma tm_subst_eq : forall u v j,
+  tm j (subst u v) = Lc.subst (tm j u) (tm (Lc.ilift j) v).
+intros.
+unfold Lc.subst; rewrite <- tm_substitutive.
+destruct v as [v|]; simpl; trivial.
+rewrite I.lams0.
+rewrite I.shift0.
+apply itm_morph.
+apply I.cons_ext; simpl.
+ rewrite Lc.lift0; trivial.
+
+ do 2 red; unfold I.shift; simpl; intros.
+ rewrite Lc.simpl_subst; trivial; rewrite Lc.lift0; trivial.
+Qed.
+
+Instance App_morph : Proper (eq_trm ==> eq_trm ==> eq_trm) App.
+unfold App; do 3 red; simpl; split; intros.
+ red; intros.
+ rewrite H; rewrite H0; rewrite H1; reflexivity.
+
+ red; intros.
+ rewrite H; rewrite H0; rewrite H1; reflexivity.
+Qed.
+
+Instance Abs_morph : Proper (eq_trm ==> eq_trm ==> eq_trm) Abs.
+unfold Abs; do 4 red; simpl; split; red; intros.
+ apply lam_ext.
+  apply int_morph; auto.
+
+  red; intros.
+  rewrite H0; rewrite H1; rewrite H3; reflexivity.
+
+ rewrite H0; rewrite H1; rewrite H; reflexivity.
+Qed.
+
+
+Instance Prod_morph : Proper (eq_trm ==> eq_trm ==> eq_trm) Prod.
+unfold Prod; do 4 red; simpl; split; red; intros.
+ apply prod_ext.
+  rewrite H; rewrite H1; reflexivity.
+
+  red; intros.
+  rewrite H0; rewrite H1; rewrite H3; reflexivity.
+
+ rewrite H0; rewrite H1; rewrite H; reflexivity.
+Qed.
+
+
+Lemma discr_ref_prod : forall n A B,
+  ~ eq_trm (Ref n) (Prod A B).
+red; intros.
+simpl in H.
+destruct H as (_,H).
+red in H.
+specialize H with Lc.Ref Lc.Ref.
+discriminate H.
+reflexivity.
+Qed.
+
+Lemma eq_trm_lift_ref_fv n k i :
+  k <= i ->
+  eq_trm (lift_rec n k (Ref i)) (Ref (n+i)).
+split; simpl; red; intros.
+ unfold V.lams.
+ destruct (le_gt_dec k i).
+  unfold V.shift; simpl.
+  replace (n+i) with (k+(n+(i-k))); auto with *.
+
+  omega.
+
+ unfold I.lams.
+ destruct (le_gt_dec k i).
+  unfold I.shift; simpl.
+  replace (n+i) with (k+(n+(i-k))); auto with *.
+
+  omega.
+Qed.
+
+(*
+Lemma lift1var : forall n, eq_trm (lift 1 (Ref n)) (Ref (S n)).
+simpl; split; red; intros.
+ revert n.
+ change (eq_val (V.lams 0 (V.shift 1) x) (V.shift 1 y)).
+ rewrite V.lams0; rewrite <- H.
+ reflexivity.
+
+ revert n.
+ change (Lc.eq_intt (I.lams 0 (I.shift 1) x) (I.shift 1 y)).
+ rewrite I.lams0; rewrite <- H.
+ reflexivity.
+Qed.
+*)
+
+Lemma red_lift_app n A B k :
+  eq_trm (lift_rec n k (App A B)) (App (lift_rec n k A) (lift_rec n k B)).
+red; simpl; intros.
+split.
+ red; intros.
+ apply app_ext.
+  rewrite int_lift_rec_eq.
+  rewrite H; reflexivity.
+
+  rewrite int_lift_rec_eq.
+  rewrite H; reflexivity.
+
+ red; intros.
+ do 2 rewrite tm_lift_rec_eq.
+ rewrite H; trivial.
+Qed.
+
+Lemma red_lift_abs n A B k :
+  eq_trm (lift_rec n k (Abs A B)) (Abs (lift_rec n k A) (lift_rec n (S k) B)).
+red; simpl; intros.
+split.
+ red; intros.
+ apply lam_ext.
+  rewrite int_lift_rec_eq.
+  rewrite H; reflexivity.
+
+  red; intros.
+  rewrite int_lift_rec_eq.
+  rewrite <- V.cons_lams.
+   rewrite H1.
+   rewrite H.
+   reflexivity.
+
+   do 2 red; intros.
+   rewrite H2; reflexivity.
+
+ red; intros.
+ apply f_equal2.
+  rewrite tm_lift_rec_eq.
+  rewrite H; auto.
+
+  rewrite tm_lift_rec_eq.
+  apply tm_morph; auto with *.
+  rewrite H.
+  apply Lc.cross_binder_shift.
+Qed.
+
+Lemma red_lift_prod n A B k :
+  eq_trm (lift_rec n k (Prod A B)) (Prod (lift_rec n k A) (lift_rec n (S k) B)).
+red; simpl; intros.
+split.
+ red; intros.
+ apply prod_ext.
+  rewrite int_lift_rec_eq.
+  rewrite H; reflexivity.
+
+  red; intros.
+  rewrite int_lift_rec_eq.
+  rewrite <- V.cons_lams.
+   rewrite H1.
+   rewrite H.
+   reflexivity.
+
+   do 2 red; intros.
+   rewrite H2; reflexivity.
+
+ red; intros.
+ apply f_equal2.
+  rewrite tm_lift_rec_eq.
+  rewrite H; auto.
+
+  rewrite tm_lift_rec_eq.
+  apply tm_morph; auto with *.
+  rewrite H.
+  apply Lc.cross_binder_shift.
+Qed.
+
+Lemma red_sigma_app N A B k :
+  eq_trm (subst_rec N k (App A B)) (App (subst_rec N k A) (subst_rec N k B)).
+red; simpl; intros.
+split.
+ red; intros.
+ apply app_ext.
+  rewrite int_subst_rec_eq.
+  rewrite H; reflexivity.
+
+  rewrite int_subst_rec_eq.
+  rewrite H; reflexivity.
+
+ red; intros.
+ do 2 rewrite tm_subst_rec_eq.
+ rewrite H; trivial.
+Qed.
+
+Lemma red_sigma_abs N A B k :
+  eq_trm (subst_rec N k (Abs A B)) (Abs (subst_rec N k A) (subst_rec N (S k) B)).
+red; simpl; intros.
+split.
+ red; intros.
+ apply lam_ext.
+  rewrite int_subst_rec_eq.
+  rewrite H; reflexivity.
+
+  red; intros.
+  rewrite int_subst_rec_eq.
+  rewrite <- V.cons_lams.
+   rewrite H1.
+   rewrite H.
+   reflexivity.
+
+   do 2 red; intros.
+   rewrite H2; reflexivity.
+
+ red; intros.
+ apply f_equal2.
+  rewrite tm_subst_rec_eq.
+  rewrite H; auto.
+
+  rewrite tm_subst_rec_eq.
+  apply tm_morph; auto with *.
+  rewrite H.
+  apply Lc.cross_binder_cons.
+  unfold I.shift, Lc.ilift; simpl.
+  unfold Lc.lift; rewrite <- tm_liftable; trivial.
+Qed.
+
+Lemma red_sigma_prod N A B k :
+  eq_trm (subst_rec N k (Prod A B)) (Prod (subst_rec N k A) (subst_rec N (S k) B)).
+red; simpl; intros.
+split.
+ red; intros.
+ apply prod_ext.
+  rewrite int_subst_rec_eq.
+  rewrite H; reflexivity.
+
+  red; intros.
+  rewrite int_subst_rec_eq.
+  rewrite <- V.cons_lams.
+   rewrite H1.
+   rewrite H.
+   reflexivity.
+
+   do 2 red; intros.
+   rewrite H2; reflexivity.
+
+ red; intros.
+ apply f_equal2.
+  rewrite tm_subst_rec_eq.
+  rewrite H; auto.
+
+  rewrite tm_subst_rec_eq.
+  apply tm_morph; auto with *.
+  rewrite H.
+  apply Lc.cross_binder_cons.
+  unfold I.shift, Lc.ilift; simpl.
+  unfold Lc.lift; rewrite <- tm_liftable; trivial.
+Qed.
+
+Lemma red_sigma_var_eq N k :
+  N <> kind ->
+  eq_trm (subst_rec N k (Ref k)) (lift k N).
+unfold subst_rec; simpl.
+destruct N; simpl.
+2:destruct 1; trivial.
+intros _.
+split; red; intros.
+ unfold V.lams, V.shift; simpl.
+ destruct (le_gt_dec k k).
+ 2:omega.
+ replace (k-k) with 0; auto with *.
+ simpl V.cons.
+ apply iint_morph.
+ do 2 red; intros.
+ replace (a-0) with a; auto with *.
+
+ unfold I.lams; simpl.
+ destruct (le_gt_dec k k).
+ 2:omega.
+ replace (k-k) with 0; auto with *.
+ simpl I.cons.
+ apply itm_morph.
+ do 2 red; intros.
+ unfold I.shift; simpl.
+ replace (a-0) with a; auto with *.
+Qed.
+
+Lemma red_sigma_var_lt N k n :
+  n < k ->
+  eq_trm (subst_rec N k (Ref n)) (Ref n).
+unfold subst_rec; simpl; intros.
+split; red; intros.
+ unfold V.lams, V.shift; simpl.
+ destruct (le_gt_dec k n); auto.
+ omega.
+
+ unfold I.lams, I.shift; simpl.
+ destruct (le_gt_dec k n); auto.
+ omega.
+Qed.
+
+Lemma red_sigma_var_gt N k n :
+  k <= n ->
+  eq_trm (subst_rec N k (Ref (S n))) (Ref n).
+unfold subst_rec; simpl; intros.
+split; red; intros.
+ unfold V.lams; simpl.
+ destruct (le_gt_dec k (S n)); simpl.
+  unfold V.cons, V.shift; simpl.
+  destruct k; simpl; auto.
+  replace (n-k) with (S (n-S k)).
+   replace (S (k+(n- S k))) with n; auto.
+   omega.
+  omega.
+ omega.
+
+ unfold I.lams, I.shift, I.cons; simpl.
+ destruct (le_gt_dec k (S n)); simpl.
+  destruct k; simpl; auto.
+  replace (n-k) with (S (n-S k)).
+   replace (S (k+(n- S k))) with n; auto.
+   omega.
+  omega.
+ omega.
+Qed.
+
+Lemma simpl_subst_lift_rec A M k :
+  eq_trm M (subst_rec A k (lift_rec 1 k M)).
+destruct M;[|exact I].
+simpl; split; red; intros.
+ apply iint_morph; do 2 red; intros.
+ unfold V.lams, V.shift, V.cons; simpl.
+ destruct (le_gt_dec k a); auto.
+ destruct le_gt_dec.
+ 2:omega.
+ case_eq (k+S(a-k)-k); intros. 
+  omega.
+
+  replace a with (k+n); auto.
+  omega.
+
+ apply itm_morph; do 2 red; intros.
+ unfold I.lams, I.shift, I.cons; simpl.
+ destruct (le_gt_dec k a); auto.
+ destruct le_gt_dec.
+ 2:omega.
+ case_eq (k+S(a-k)-k); intros. 
+  omega.
+
+  replace a with (k+n); auto.
+  omega.
+Qed.
+
+
+
+(* "Untyped" reduction: tools for proving simulation and strong normalization *)
+
+Definition red_term M N :=
+  forall j, Lc.redp (tm j M) (tm j N).
+
+Instance red_term_morph : Proper (eq_trm ==> eq_trm ==> iff) red_term.
+apply morph_impl_iff2; auto with *.
+do 4 red; intros.
+red; intros.
+rewrite <- H; rewrite <- H0; auto.
+Qed.
+
+Lemma red_term_trans M1 M2 M3 :
+  red_term M1 M2 -> red_term M2 M3 -> red_term M1 M3.
+unfold red_term; intros.
+specialize H with j.
+specialize H0 with j.
+apply t_trans with (tm j M2); trivial.
+Qed.
+
+Lemma red_term_app_l M M' N :
+  red_term M M' ->
+  red_term (App M N) (App M' N).
+unfold red_term; intros.
+specialize H with j.
+apply Lc.redp_app_l; trivial.
+Qed.
+
+Lemma red_term_app_r M N N' :
+  red_term N N' ->
+  red_term (App M N) (App M N').
+unfold red_term; intros.
+specialize H with j.
+apply Lc.redp_app_r; trivial.
+Qed.
+
+Lemma red_term_abs_l M M' N :
+  red_term M M' ->
+  red_term (Abs M N) (Abs M' N).
+unfold red_term; intros.
+specialize H with j.
+simpl.
+apply Lc.redp_app_r; trivial.
+Qed.
+
+Lemma red_term_abs_r M N N' :
+  red_term N N' ->
+  red_term (Abs M N) (Abs M N').
+unfold red_term; intros.
+specialize H with (Lc.ilift j).
+simpl.
+apply Lc.redp_app_l; trivial.
+apply Lc.redp_app_r; trivial.
+apply Lc.redp_abs; trivial.
+Qed.
+
+Lemma red_term_prod_l M M' N :
+  red_term M M' ->
+  red_term (Prod M N) (Prod M' N).
+unfold red_term; intros.
+specialize H with j.
+simpl.
+apply Lc.redp_app_l; trivial.
+apply Lc.redp_app_r; trivial.
+Qed.
+
+Lemma red_term_prod_r M N N' :
+  red_term N N' ->
+  red_term (Prod M N) (Prod M N').
+unfold red_term; intros.
+specialize H with (Lc.ilift j).
+simpl.
+apply Lc.redp_app_r; trivial.
+apply Lc.redp_abs; trivial.
+Qed.
+
+Lemma red_term_beta T M N :
+  red_term (App (Abs T M) N) (subst N M).
+red; simpl; intros.
+eapply t_trans.
+ eapply Lc.redp_app_l.
+ eapply Lc.redp_K.
+
+ apply t_step.
+ apply Lc.red1_beta.
+ unfold Lc.subst; rewrite <- tm_substitutive.
+ destruct M; simpl; trivial.
+ rewrite I.lams0.
+ unfold I.shift; simpl.
+ apply itm_morph.
+ do 2 red; intros.
+ destruct a; simpl.
+  rewrite Lc.lift0; trivial.
+
+  rewrite Lc.simpl_subst; auto.
+  rewrite Lc.lift0; trivial.
+Qed.
+
+(* This lemma shows that the strong normalization of any
+   term interpretation entails the strong normalization
+   of the original "term" (w.r.t. red_trans).
+ *)
+Lemma simul M :
+  Lc.sn M ->
+  forall j M', M = tm j M' ->
+  Acc (transp _ red_term) M'.
+intros snM.
+elim (Acc_clos_trans _ _ _ snM); clear snM; intros.
+constructor; intros.
+red in H2.
+assert (redM' := H2 j).
+assert (clos_trans _ (transp _ Lc.red1) (tm j y) x).
+ rewrite H1.
+ clear H1 H2.
+ elim redM'; intros.
+  apply t_step; trivial.
+
+  apply t_trans with y0; trivial.
+apply H0 with (tm j y) j; trivial.
+Qed.
+
+
+(* Iterated products *)
+
+Fixpoint prod_list (e:list trm) (U:trm) :=
+  match e with
+  | List.nil => U
+  | T::f => Prod T (prod_list f U)
+  end.
+
+Lemma lift_prod_list_ex n k e T :
+  exists e',
+  eq_trm (lift_rec n k (prod_list e T))
+    (prod_list e' (lift_rec n (length e+k) T)).
+revert k; induction e; intros.
+ exists nil; reflexivity.
+
+ destruct (IHe (S k)) as (e',?).
+ exists (cons (lift_rec n k a) e').
+ simpl prod_list.
+ rewrite red_lift_prod.
+ rewrite H.
+ replace (length e + S k) with (S (length e +k)); auto with *.
+Qed.
+Lemma subst_prod_list_ex M k e T :
+  exists e',
+  eq_trm (subst_rec M k (prod_list e T))
+    (prod_list e' (subst_rec M (length e+k) T)).
+revert k; induction e; intros.
+ exists nil; reflexivity.
+
+ destruct (IHe (S k)) as (e',?).
+ exists (cons (subst_rec M k a) e').
+ simpl prod_list.
+ rewrite red_sigma_prod.
+ rewrite H.
+ replace (length e + S k) with (S (length e +k)); auto with *.
+Qed.
+
+
+End MakeObject.
